@prefix : <http://ontology.causeex.com/ontology/odps/TimeSeriesAndMeasurements#> .
@prefix cco: <http://www.ontologyrepository.com/CommonCoreOntologies/> .
@prefix dcterms: <http://purl.org/dc/terms/> .
@prefix meas: <http://ontology.causeex.com/ontology/odps/TimeSeriesAndMeasurements#> .
@prefix owl: <http://www.w3.org/2002/07/owl#> .
@prefix rdf: <http://www.w3.org/1999/02/22-rdf-syntax-ns#> .
@prefix rdfs: <http://www.w3.org/2000/01/rdf-schema#> .
@prefix xsd: <http://www.w3.org/2001/XMLSchema#> .

<http://ontology.causeex.com/ontology/odps/MeasurementUnits> rdf:type owl:Ontology ;
    dcterms:created "April 16, 2018"^^xsd:string ;
    dcterms:modified "October 5, 2018"^^xsd:string ;
    dcterms:description "Ontology holding new classes and individuals, extending the hierarchy and taxonomy of the CCO UnitsOfMeasure ontology."@en ;
    rdfs:comment """October 5th 2018 revisions:
                    Updated the imports to only inclue what is explicitly referenced.
                  August 3rd 2018 revisions:
                    Added the import of the TimeSeriesAndMeasurements ontology, for completeness.
                  May 24th 2018 revisions:
                    Added an rdfs:comment for NumberMeasurementUnit.
                  April 30th 2018 revision:
                    Added NumberMeasurementUnit."""@en ;
#   owl:imports <http://www.ontologyrepository.com/CommonCoreOntologies/Mid/AllCoreOntology> ;
    owl:imports <http://www.ontologyrepository.com/CommonCoreOntologies/Mid/ArtifactOntology> ;
    owl:imports <http://www.ontologyrepository.com/CommonCoreOntologies/Upper/ExtendedRelationOntology> ;
    owl:imports <http://www.ontologyrepository.com/CommonCoreOntologies/Mid/UnitsOfMeasureOntology> ;
    owl:imports <http://ontology.causeex.com/ontology/odps/TimeSeriesAndMeasurements> ;
    owl:imports <http://purl.org/dc/terms> ;
    owl:versionInfo "Version 0.6"^^xsd:string .


#################################################################
#    Classes
#################################################################

:MeasurementUnitOfAmount a owl:Class ;
    rdfs:label "Measurement Unit of Amount"@en ;
    rdfs:subClassOf cco:MeasurementUnit ;
    rdfs:comment "A Measurement Unit used in chemistry to express the amounts of reactants and products of chemical reactions."@en ;
    cco:example_of_usage "mole"^^xsd:string .

:MeasurementUnitOfCatalyticActivity a owl:Class ;
    rdfs:label "Measurement Unit of Catalytic Activity"@en ;
    rdfs:subClassOf cco:MeasurementUnit ;
    rdfs:comment "A Measurement Unit used to quantify catalytic activity."@en ;
    cco:example_of_usage "katal"^^xsd:string .

:MeasurementUnitOfElectromagnetism a owl:Class ;
    rdfs:label "Measurement Unit of Electromagnetism"@en ;
    rdfs:subClassOf cco:MeasurementUnit ;
    rdfs:comment "A Measurement Unit used with systems of electrical units, based on the magnetic properties of electric currents."@en ;
    cco:example_of_usage "amperes, volts"^^xsd:string .

:MeasurementUnitOfPhotometry a owl:Class ;
    rdfs:label "Measurement Unit of Photometry"@en ;
    rdfs:subClassOf cco:MeasurementUnit ;
    rdfs:comment "A Measurement Unit used in photometry, related to light and how it is perceived."@en ;
    cco:example_of_usage "candela, lumen"^^xsd:string .

:MeasurementUnitOfRadioactivity a owl:Class ;
    rdfs:label "Measurement Unit of Radioactivity"@en ;
    rdfs:subClassOf cco:MeasurementUnit ;
    rdfs:comment "A Measurement Unit used to report radioactive decay and exposures/dosages."@en ;
    cco:example_of_usage "becquerel, gray"^^xsd:string .


#################################################################
#    Individuals
#################################################################

:AmpereMeasurementUnit a owl:NamedIndividual, :MeasurementUnitOfElectromagnetism ;
    rdfs:label "Ampere Measurement Unit" .

:BecquerelMeasurementUnit a owl:NamedIndividual, :MeasurementUnitOfRadioactivity ;
    rdfs:label "Becquerel Measurement Unit" .

:CandelaMeasurementUnit a owl:NamedIndividual, :MeasurementUnitOfPhotometry ;
    rdfs:label "Candela Measurement Unit" .

:CoulombMeasurementUnit a owl:NamedIndividual, :MeasurementUnitOfElectromagnetism ;
    rdfs:label "Coulomb Measurement Unit" .

:DaltonMeasurementUnit a owl:NamedIndividual, cco:MeasurementUnitOfMass ;
    rdfs:label "Dalton Measurement Unit" .

:ElectronvoltMeasurementUnit a owl:NamedIndividual, cco:MeasurementUnitOfEnergy ;
    rdfs:label "Electronvolt Measurement Unit" .

:FaradMeasurementUnit a owl:NamedIndividual, :MeasurementUnitOfElectromagnetism ;
    rdfs:label "Farad Measurement Unit" .

:GrayMeasurementUnit a owl:NamedIndividual, :MeasurementUnitOfRadioactivity ;
    rdfs:label "Gray Measurement Unit" .

:HenryMeasurementUnit a owl:NamedIndividual, :MeasurementUnitOfElectromagnetism ;
    rdfs:label "Henry Measurement Unit" .

:KatalMeasurementUnit a owl:NamedIndividual, :MeasurementUnitOfCatalyticActivity ;
    rdfs:label "Katal Measurement Unit" .

:KelvinMeasurementUnit a owl:NamedIndividual, cco:MeasurementUnitOfTemperature ;
    rdfs:label "Kelvin Measurement Unit" .

:LumenMeasurementUnit a owl:NamedIndividual, :MeasurementUnitOfPhotometry ;
    rdfs:label "Lumen Measurement Unit" .

:LuxMeasurementUnit a owl:NamedIndividual, :MeasurementUnitOfPhotometry ;
    rdfs:label "Lux Measurement Unit" .

:MoleMeasurementUnit a owl:NamedIndividual, :MeasurementUnitOfAmount ;
    rdfs:label "Mole Measurement Unit" .

:NumberMeasurementUnit a owl:NamedIndividual, :MeasurementUnitOfAmount ;
    rdfs:label "Number Measurement Unit" ;
    rdfs:comment "A count (i.e., 'number') of individuals, pieces, etc. This can define quantities such as a 'dozen eggs' by indicating the NumberMeasurementUnit and a meas:mulitplier of 12. Or, a 'baker's dozen' has a multiplier of 13."@en .

:OhmMeasurementUnit a owl:NamedIndividual, :MeasurementUnitOfElectromagnetism ;
    rdfs:label "Ohm Measurement Unit" .

:SiemensMeasurementUnit a owl:NamedIndividual, :MeasurementUnitOfElectromagnetism ;
    rdfs:label "Siemens Measurement Unit" .

:SievertMeasurementUnit a owl:NamedIndividual, :MeasurementUnitOfRadioactivity ;
    rdfs:label "Sievert Measurement Unit" .

:SteradianMeasurementUnit a owl:NamedIndividual, cco:MeasurementUnitOfAngle ;
    rdfs:label "Steradian Measurement Unit" .

:TeslaMeasurementUnit a owl:NamedIndividual, :MeasurementUnitOfElectromagnetism ;
    rdfs:label "Tesla Measurement Unit" .

:VoltMeasurementUnit a owl:NamedIndividual, :MeasurementUnitOfElectromagnetism ;
    rdfs:label "Volt Measurement Unit" .

:WattHourMeasurementUnit a owl:NamedIndividual, cco:MeasurementUnitOfEnergy ;
    rdfs:label "Watt-hour Measurement Unit" .

:WeberMeasurementUnit a owl:NamedIndividual, :MeasurementUnitOfElectromagnetism ;
    rdfs:label "Weber Measurement Unit" .
