@prefix : <http://ontology.causeex.com/ontology/odps/TimeSeriesAndMeasurements#> .
@prefix cco: <http://www.ontologyrepository.com/CommonCoreOntologies/> .
@prefix dcterms: <http://purl.org/dc/terms/> .
@prefix event: <http://ontology.causeex.com/ontology/odps/Event#> .
@prefix general: <http://ontology.causeex.com/ontology/odps/GeneralConcepts#> .
@prefix meas: <http://ontology.causeex.com/ontology/odps/TimeSeriesAndMeasurements#> .
@prefix owl: <http://www.w3.org/2002/07/owl#> .
@prefix rdf: <http://www.w3.org/1999/02/22-rdf-syntax-ns#> .
@prefix rdfs: <http://www.w3.org/2000/01/rdf-schema#> .
@prefix xml: <http://www.w3.org/XML/1998/namespace> .
@prefix xsd: <http://www.w3.org/2001/XMLSchema#> .

<http://ontology.causeex.com/ontology/odps/TimeSeriesAndMeasurements> rdf:type owl:Ontology ;
    dcterms:created "April 16, 2018"^^xsd:string ;
    dcterms:modified "October 22, 2018"^^xsd:string ;
    rdfs:comment """October 22nd 2018 revisions:
                    Changed the sub-classing of TimeSeries (from owl:Thing) to be event:CollectionOfEvents.
                    Removed ReportedProperty, its sub-class hierarchy and the defined_by property (not needed with the new sub-classing
                      of TimeSeries/ReportedValue and the alignment of the ReportedProperty sub-classes into the Event hierarchy).
                    Added the SeriesTrend class, its individual values and the has_trend object property.
                    Removed has_time_series as this is not needed (the properties, general:located_at and is_about_xxx can be used instead).
                    Renamed has_property_type to has_value_type and declared it as a FunctionalProperty. 
                    Removed the reported_event_class_string property since its semantics are addressed in the ICM ontology.
                    Removed the MonetaryAmountPrice individual as it is not used.
                    Corrected comments related to decimal_value (changed to numeric_value) and removed references to is_about_using_artifact.
                  September 24th 2018 revisions:
                    Changed rdfs:Literal to xsd:string, xsd:float to xsd:decimal or xsd:double, and also allowed xsd:decimal with xsd:double.
                  July 29th revisions:
                    Clarified the usage of is_about_artifact, and removed is_about_using_artifact.
                  June 19th 2018 revisions:
                    Added is_about_actor and the ranges of the general:associate_monetary_amount property.
                    Corrected the range for the minimum/maximum_numeric_values (incorrectly still set to xsd:decimal).
                    Added a domain definition for general:has_currency.
                    Added the TextEnum individual and the enum_value property.
                  May 2nd 2018 revisions:
                    Renamed decimal_value and minimum/maximum_decimal_value to numeric_value and minimum/maximum_numeric_value 
                       (all defined as decimals or doubles to allow more flexibility).
                    Added that general:has_currency is a sub-property of has_measurement_unit."""@en ;
#   owl:imports <http://www.ontologyrepository.com/CommonCoreOntologies/Mid/AllCoreOntology> ;
    owl:imports <http://www.ontologyrepository.com/CommonCoreOntologies/Mid/ArtifactOntology> ;
    owl:imports <http://www.ontologyrepository.com/CommonCoreOntologies/Mid/UnitsOfMeasureOntology> ;
    owl:imports <http://ontology.causeex.com/ontology/odps/Event> ;
    owl:imports <http://ontology.causeex.com/ontology/odps/GeneralConcepts> ;
    owl:imports <http://purl.org/dc/terms> ;
    owl:versionInfo "Version 1.0"^^xsd:string .


#################################################################
#    Object Properties
#################################################################

:has_increased_value a owl:ObjectProperty, owl:IrreflexiveProperty, owl:TransitiveProperty ;
    rdfs:label "has increased value"@en ;
    rdfs:comment "Property associating two ReportedValues indicating that the value is increasing when comparing the source/subject to the target/object. This information is useful if specific value information is not available, but the direction of change is known."@en ; 
    rdfs:domain :ReportedValue ;
    rdfs:range :ReportedValue .

:has_measurement_unit a owl:ObjectProperty, owl:FunctionalProperty ;
    rdfs:label "has measurement unit"@en ;
    rdfs:comment "Indicates the units in which a ReportedValue or all the ReportedValues in a TimeSeries are expressed. To define the units for all the Values in a TimeSeries, the has_measurement_unit property is specified at the level of the TimeSeries. Otherwise, it is defined for the individual ReportedValues. The units are specified as one of the individuals in the CCO UnitsOfMeasure or Measurements-Units ontologies."@en ;
    rdfs:domain _:UnionOfTimeSeriesReportedValue ;
    rdfs:range cco:MeasurementUnit .
general:has_currency rdfs:subPropertyOf :has_measurement_unit ;
    rdfs:domain _:UnionOfTimeSeriesReportedValue .

:has_relative_unit a owl:ObjectProperty, owl:FunctionalProperty ;
    rdfs:label "has relative unit"@en ;
    rdfs:comment "If a measurement unit is defined as a ratio such as 'x per liter', 'x per hour' or a similar value, then the second unit is specified using the meas:has_relative_unit property. To define the units for all the Values in a TimeSeries, the has_measurement_unit property is specified at the level of the TimeSeries. Otherwise, it is defined for the individual ReportedValues. The units are specified as one of the individuals in the CCO UnitsOfMeasure or Measurements-Units ontologies."@en ; 
    rdfs:domain _:UnionOfTimeSeriesReportedValue ;
    rdfs:range cco:MeasurementUnit .

:has_reported_value a owl:ObjectProperty, owl:IrreflexiveProperty ;
    rdfs:label "has reported value"@en ;
    rdfs:comment "Property describing that a TimeSeries 'aggregates' the ReportedValues referenced by this property, or that an Event/Factor is related to the ReportedValue. (Since a TimeSeries is a sub-class of event:CollectionOfEvents, which is itself an Event, setting the domain of this property to event:Event addresses both uses discussed in the previous sentence.)"@en ; 
    rdfs:domain event:Event ;
    rdfs:range :ReportedValue .
general:associated_monetary_amount rdfs:subPropertyOf :has_reported_value .

:has_same_value a owl:ObjectProperty, owl:IrreflexiveProperty, owl:TransitiveProperty ;
    rdfs:label "has same value"@en ;
    rdfs:comment "Property associating two ReportedValues indicating that the value is relatively the same when comparing the source/subject to the target/object. This information is useful if specific value information is not available, but the fact that no change occurred is known."@en ; 
    rdfs:domain :ReportedValue ;
    rdfs:range :ReportedValue .

:has_trend a owl:ObjectProperty, owl:FunctionalProperty ;
    rdfs:label "has trend"@en ;
    rdfs:comment "Indicates the trend of a TimeSeries or the trend at the specific point in time of a ReportedValue."@en ;
    rdfs:domain _:UnionOfTimeSeriesReportedValue ;
    rdfs:range :SeriesTrend .

:has_value1 a owl:ObjectProperty, owl:FunctionalProperty ;
    rdfs:label "has value1"@en ;
    rdfs:comment "Two values are associated with a RelatedValues individual - value1 and value2. The two are 'related' by a factor specified by the RelatedValues ratio property where ratio * value2 = value1. This sort of definition is needed when text specifies that a value is 'up 7 percent from a year ago', or some similar ratio, but the exact value is not known. For the example of 'up 7 percent', the ratio would be 1.07."@en ; 
    rdfs:domain :RelatedValues ;
    rdfs:range :ReportedValue .

:has_value2 a owl:ObjectProperty, owl:FunctionalProperty ;
    rdfs:label "has value2"@en ;
    rdfs:comment "Two values are associated with a RelatedValues individual - value1 and value2. The two are 'related' by a factor specified by the RelatedValues ratio property where ratio * value2 = value1. This sort of definition is needed when text specifies that a value is 'up 7 percent from a year ago', or some similar ratio, but the exact value is not known. For the example of 'up 7 percent', the ratio would be 1.07."@en ; 
    rdfs:domain :RelatedValues ;
    rdfs:range :ReportedValue .

:has_value_type a owl:ObjectProperty, owl:FunctionalProperty ;
    rdfs:label "has value type"@en ;
    rdfs:comment "Property defining whether a ReportedValue's quantity/quality is a count, percentage, average, raw value, rank, index or enumerated value. The ReportedValueType, which is the range of this property, is a closed enumeration containing seven individuals with these semantics."@en ; 
    rdfs:comment "If the ReportedValueType varies at the level of the individual ReportedValues, then the has_value_type property should be associated with each ReportedValue (even if the Values are in a TimeSeries). If the ValueType is the same for all the ReportedValues in a TimeSeries, then the property can be defined once, for the TimeSeries."@en ;
    rdfs:domain _:UnionOfTimeSeriesReportedValue ;
    rdfs:range :ReportedValueType .

:is_about_actor a owl:ObjectProperty ;
    rdfs:label "is about actor"@en ;
    rdfs:comment "Property indicating that the semantics of the referencing TimeSeries or ReportedValue are about a specific type of actor (typically, a GroupOfPersons such as Refugees or DisplacedPersons). For example, a TimeSeries may describe the average number of DisplacedPersons from a country, over some time period. These semantics are 'about' the group (an individual of type, actor:DisplacedPersons). The group would be related to the TimeSeries using the meas:is_about_actor property."@en ;
    rdfs:comment "It may happen that an actor associated with a TimeSeries is further refined by a ReportedValue (in the series). This could occur if, for example, the TimeSeries is about the average number (demographics) of DisplacedPersons from a country, but the individual values are about the average number of different ethnicities. This detail can be captured by using the meas:is_about_actor property at both the TimeSeries and ReportedValue levels."@en ;
    rdfs:domain _:UnionOfTimeSeriesReportedValue ;
    rdfs:range event:Actor ;
    rdfs:subPropertyOf event:has_actor .

:is_about_artifact a owl:ObjectProperty ;
    rdfs:label "is about artifact"@en ;
    rdfs:comment "Property indicating that the semantics of the referencing TimeSeries or ReportedValue deal with a specific artifact. For example, it may happen that a generic artifact (like food) is associated with a TimeSeries (for example, describing the average price of food) and that is further refined by its ReportedValues. In this case, the TimeSeries can be classified as event:Pricing, with the meas:is_about_artifact referencing event:Food, but the individual ReportedValues are about the average price of milk, eggs, meat, .... This detail can be captured by using is_about_artifact at the ReportedValue level. In this case, meas:is_about_artifact references some individual of type, event:Food and event:SpecificTypeOfArtifact. The individual's rdfs:label then defines 'milk', 'eggs', 'meat', etc."@en ;
    rdfs:comment "Alternately, it may happen that an artifact (such as the price of transportation by bus) is associated with a TimeSeries, and is also further refined by its ReportedValues. In this case, the TimeSeries is classified as event:Pricing and event:PersonalTransportation, and meas:is_about_artifact references cco:Bus (clarifying the type of transportation). If the individual ReportedValues are about the average prices of intra- and inter-city busses, that distinction can be captured by using the is_about_artifact property at the ReportedValue level (using a similar technique as discussed above)."@en ;
    rdfs:domain _:UnionOfTimeSeriesReportedValue ;
    rdfs:range cco:Artifact ;
    rdfs:subPropertyOf event:is_about_artifact .


#################################################################
#    Data Properties
#################################################################

:divisor a owl:DatatypeProperty, owl:FunctionalProperty ;
    rdfs:label "divisor"@en ;
    rdfs:comment "If a measurement unit is defined in units of mg or mm (milligrams or millimeters), then the divisor for the 'base' unit (in this case, grams or meters) can be specified. It is expressed as an xsd:decimal or xsd:double using this property. To define the divisor for all the Values in a TimeSeries, this property is specified at the level of the TimeSeries. Otherwise, it is defined for the individual ReportedValues."@en ;
    rdfs:comment "It is recommended that unit information extracted from the source documents always be converted to 'base' units. 'Base' units are units of measure without any prefix (such as 'kilo', 'giga', 'tera', 'milli', 'nano', ...). Examples of 'base' units are gram, second and mile. These are enumerated in the CCO UnitsOfMeasure Ontology, and extended in the Measurements-Units ontology. A divisor datatype property allows expressing prefixes without requiring the creation of hundreds of variations of the base units."@en ; 
    rdfs:domain _:UnionOfTimeSeriesReportedValue ;
    rdfs:range [ a rdfs:Datatype ;
                 owl:unionOf ( xsd:decimal xsd:double ) ] .

:enum_value a owl:DatatypeProperty, owl:FunctionalProperty ;
    rdfs:label "enumerated value"@en ;
    rdfs:comment "A string specifying the value of a ReportedValue individual, when its ReportedValueType is TextEnum."@en ;
    rdfs:domain :ReportedValue ;
    rdfs:range xsd:string .

:maximum_numeric_value a owl:DatatypeProperty, owl:FunctionalProperty ;
    rdfs:label "maximum numeric value"@en ;
    rdfs:comment "An xsd:decimal or xsd:double specifying the largest/maximum possible amount/measurement/observation of a ReportedValue individual."@en ;
    rdfs:domain :ReportedValue ;
    rdfs:range [ a rdfs:Datatype ;
                 owl:unionOf ( xsd:decimal xsd:double ) ] .
general:largest_possible_amount rdfs:subPropertyOf :maximum_numeric_value .

:minimum_numeric_value a owl:DatatypeProperty, owl:FunctionalProperty ;
    rdfs:label "minimum numeric value"@en ;
    rdfs:comment "An xsd:decimal or xsd:double specifying the smallest/minimum possible amount/measurement/observation of a ReportedValue individual."@en ;
    rdfs:domain :ReportedValue ;
    rdfs:range [ a rdfs:Datatype ;
                 owl:unionOf ( xsd:decimal xsd:double ) ] .
general:smallest_possible_amount rdfs:subPropertyOf :minimum_numeric_value .

:multiplier a owl:DatatypeProperty, owl:FunctionalProperty ;
    rdfs:label "multiplier"@en ;
    rdfs:comment "If a measurement unit is defined in units of Kg or Km (kilograms or kilometers), then the multiplier for the 'base' unit (in this case, grams or meters) can be specified. It is expressed as an xsd:decimal or xsd:double using this property. To define the multiplier for all the Values in a TimeSeries, this property is specified at the level of the TimeSeries. Otherwise, it is defined for the individual ReportedValues."@en ;
    rdfs:comment "It is recommended that unit information extracted from the source documents always be converted to 'base' units. 'Base' units are units of measure without any prefix (such as 'kilo', 'giga', 'tera', 'milli', 'nano', ...). Examples of 'base' units are gram, second and mile. These are enumerated in the CCO UnitsOfMeasure Ontology, and extended in the Measurements-Units ontology. A multiplier datatype property allows expressing prefixes without requiring the creation of hundreds of variations of the base units."@en ; 
    rdfs:domain _:UnionOfTimeSeriesReportedValue ;
    rdfs:range [ a rdfs:Datatype ;
                 owl:unionOf ( xsd:decimal xsd:double ) ] .

:numeric_value a owl:DatatypeProperty, owl:FunctionalProperty ;
    rdfs:label "numeric value"@en ;
    rdfs:comment "An xsd:decimal or xsd:double specifying the amount/measurement/observation of a ReportedValue individual."@en ;
    rdfs:domain :ReportedValue ;
    rdfs:range [ a rdfs:Datatype ;
                 owl:unionOf ( xsd:decimal xsd:double ) ] .
general:amount rdfs:subPropertyOf :numeric_value .

:ratio a owl:DatatypeProperty, owl:FunctionalProperty ;
    rdfs:label "ratio"@en ;
    rdfs:comment "A decimal indicating the ratio between the two values associated to a RelatedValues individual (i.e., the ratio is equal to value1/value2). This sort of definition is needed when text specifies that a value is 'up 7 percent from a year ago', or some similar ratio, but the exact value is not known. For the example of 'up 7 percent', the ratio would be 1.07."@en ;
    rdfs:domain :RelatedValues ;
    rdfs:range xsd:decimal .

:relative_divisor a owl:DatatypeProperty, owl:FunctionalProperty ;
    rdfs:label "relative divisor"@en ;
    rdfs:comment "If a measurement unit is defined as a ratio, such as 'x per liter' or 'x per hour', then the second unit is specified using the meas:has_relative_unit property. If this unit also has a divisor, such as 'x per cm', then that divisor is expressed as an xsd:decimal or xsd:double using the relative_divisor property. To define the relative_divisor for all the Values in a TimeSeries, this property is specified at the level of the TimeSeries. Otherwise, it is defined for the individual ReportedValues."@en ;
    rdfs:domain _:UnionOfTimeSeriesReportedValue ;
    rdfs:range [ a rdfs:Datatype ;
                 owl:unionOf ( xsd:decimal xsd:double ) ] .

:relative_multiplier a owl:DatatypeProperty, owl:FunctionalProperty ;
    rdfs:label "relative multiplier"@en ;
    rdfs:comment "If a measurement unit is defined as a ration, such as 'x per liter' or 'x per hour', then the second unit is specified using the meas:has_relative_unit property. If this unit also has a multiplier, such as 'x per 1Kg', then that multiplier is expressed as an xsd:decimal or xsd:double using the relative_multiplier property. To define the relative_multiplier for all the Values in a TimeSeries, this property is specified at the level of the TimeSeries. Otherwise, it is defined for the individual ReportedValues."@en ;
    rdfs:domain _:UnionOfTimeSeriesReportedValue ;
    rdfs:range [ a rdfs:Datatype ;
                 owl:unionOf ( xsd:decimal xsd:double ) ] .


#################################################################
#    Classes
#################################################################

:RelatedValues a owl:Class ;
    rdfs:label "Related Values"@en ;
    rdfs:comment "RelatedValues exists to reify the relationship between two values - value1 and value2. The two values are 'related' by a formula specified by the RelatedValues' ratio property (where ratio * value2 = value1). This sort of definition is needed when text specifies that a value is 'up 7 percent from a year ago', or some similar ratio, but the exact value is not known. For the example of 'up 7 percent', the ratio would be 1.07."@en .

:ReportedValue a owl:Class ;
    rdfs:label "Reported Value"@en ;
    rdfs:comment "Individual ReportedValues capture specific or relative measurements/observations, and are defined using a decimal or double format (via the numeric_value datatype property) or as a string (via enum_value), along with the time when the value was measured/observed. Time is specified using the GeneralConcepts ontology's earliest/latest_possible_start/end_time properties. If an exact value cannot be reported, a range of values may be specified using the maximum/minimum_numeric_value properties, or relative values may be defined using the has_increased_value or has_same_value properties or by defining and being referenced by a RelatedValues individual."@en ;
    rdfs:comment "A ReportedValue is typically part of a TimeSeries, but it may define some specific/standalone measurement for an Event/Factor. For example, the extraction pipeline could find text indicating that the GDP of Nigeria was xx.xx NGN in 2016. If this occurs, the ReportedValue can be classified as both a meas:ReportedValue and the appropriate Event/Factor type. For this example, the additional type would be event:GrossDomesticProduct. For Values in a TimeSeries, the Series typically defines the overall semantic (event:GrossDomesticProduct, general:located_at cameo:CAMEOnga) and associates its Values using the has_reported_value property. Although not typical, a ReportedValue MAY refine the information of its TimeSeries using the general:located_at or meas:is_about_xxx properties, or refine its semantics by using a more specific type definition."@en ;
    rdfs:comment "Since a ReportedValue is a sub-class of Event, it can utilize the has_polarity property to indicate positive or negative support for the Event type."@en ;
    rdfs:comment "A ReportedValue individual may have a sourcing document component associated with it. Also, if the units in which the value is reported vary across the measurements within a time series, then the unit type, relative units and/or scale (multipliers/divisors) must be specified for each individual ReportedValue."@en ;
    rdfs:comment "Note that the trend of a ReportedValue can be specified (e.g., the trend at that particular point in time) using the has_trend object property."@en ;
    rdfs:subClassOf event:Event .
general:MonetaryAmount rdfs:subClassOf :ReportedValue .

:ReportedValueType a owl:Class ;
    rdfs:label "Reported Value Type"@en ;
    rdfs:comment "A closed enumeration consisting of the individuals: Average, Count, Index, Percentage, Rank, RawValue and TextEnum. An individual from the enumeration is associated with a TimeSeries or a ReportedValue via the has_value_type object property. It indicates how any ReportedValues in the TimeSeries or any individual ReportedValues are interpreted. If the ReportedValueType varies at the level of the individual ReportedValues, then the has_value_type property should be associated with each ReportedValue (even if the Values are in a TimeSeries). If the ValueType is the same for all the ReportedValues in a TimeSeries, then the property can be defined once, for the TimeSeries."@en ;
    rdfs:comment "Note that a type of TextEnum indicates that non-numeric values are recorded in the TimeSeries or ReportedValue, and these values are taken from some vocabulary/set of enumerated values."@en ;
    owl:equivalentClass [ a owl:Class ;
                          owl:oneOf ( :Average :Count :Percentage :RawValue :Rank :Index :TextEnum ) ] .

:SeriesTrend a owl:Class ;
    rdfs:label "Series Trend"@en ;
    rdfs:comment "An enumeration (a 'closed class') which indicates the trend of a TimeSeries overall, or the trend at the specific point in time of a ReportedValue. The value is one of :LargeDecrease, :LargeIncrease, :NoChange, :Outlier, :SmallDecrease or :SmallIncrease. A TimeSeries' or Value's trend is indicated using the has_trend property."@en ;
    owl:equivalentClass [ a owl:Class ;
                          owl:oneOf ( :LargeDecrease :LargeIncrease :NoChange :Outlier :SmallDecrease :SmallIncrease ) ] .

:TimeSeries a owl:Class ;
    rdfs:label "Time Series"@en ;
    rdfs:comment "A TimeSeries individual aggregates a set of measurements/observations, ordered by time. It consists of a set of ReportedValues (defined using the has_reported_value property), for a specific individual (where the TimeSeries defines its individual context using the general:located_at or meas:is_about_xxx properties). Examples of TimeSeries include a listing of the temperatures of a sensor at some location, the GDP of a nation over several quarters and several years, a set of percentages indicating what portion of a population supports the local government, or the percentage of contaminants in drinking water in a city."@en ;
    rdfs:comment "The semantics of a TimeSeries are defined by its meas:TimeSeries type as well as an Event type. This is valid since a TimeSeries is a sub-class of event:CollectionOfEvent (which is a sub-class of Event). So, for the four examples in the previous comment, the respective TimeSeries would be defined as individuals with type, meas:TimeSeries, as well as type(s): 1) event:PhysicalMeasurement (with a meas:has_measurement_unit property referencing cco:DegreeCelsiusMeasurementUnit or the appropriate temperature unit, with a general:located_at property referencing the sensor's location, and with a meas:has_value_type property referencing RawValue), 2) event:GrossDomesticProduct (with meas:has_measurement_unit or its sub-property, general:has_currency, referencing the appropriate currency, with a general:located_at property referencing the country, with a meas:has_value_type property referencing RawValue, and perhaps with a meas:multiplier property), 3) event:DefenseOrSupport (with a meas:has_value_type property referencing Percentage, and with a meas:is_about_actor referencing the local government, which in turn is a location and a GPE), and 4) event:EnvironmentalFactor (with a meas:has_value_type property referencing Percentage, with a general:located_at property referencing the city, and with meas:is_about_artifact properties referencing event:Water and event:ChemicalSubstance)."@en ;
    rdfs:comment "Since a TimeSeries is a sub-class of Event, it can utilize the has_polarity property to indicate positive or negative support for the Event type."@en ;
    rdfs:comment "Note that if the units for all ReportedValues in a TimeSeries are the same, then the unit type, relative units and/or scale (multipliers/divisors) can be specified for the TimeSeries individual and do not have to be repeated for each ReportedValue. The same logic applies regarding the ReportedValueType. If the Type does not vary across the ReportedValues of the TimeSeries, then it can be defined at the level of the TimeSeries and not repeated for each Value."@en ;
    rdfs:comment "Also note that the overall trend of a TimeSeries can be reported using the has_trend object property."@en ;
    rdfs:subClassOf event:CollectionOfEvents .

_:UnionOfTimeSeriesReportedValue a owl:Class ;
    owl:unionOf ( :ReportedValue :TimeSeries ) .


#################################################################
#    Individuals
#################################################################

:Average a owl:NamedIndividual, :ReportedValueType ;
    rdfs:label "Average"@en .

:Count a owl:NamedIndividual, :ReportedValueType ;
    rdfs:label "Count"@en .

:Index a owl:NamedIndividual, :ReportedValueType ;
    rdfs:label "Index"@en .

:LargeDecrease a owl:NamedIndividual, :SeriesTrend ;
    rdfs:label "Large Decrease"@en .

:LargeIncrease a owl:NamedIndividual, :SeriesTrend ;
    rdfs:label "Large Increase"@en .

:NoChange a owl:NamedIndividual, :SeriesTrend ;
    rdfs:label "No Change"@en .

:Outlier a owl:NamedIndividual, :SeriesTrend ;
    rdfs:label "Outlier"@en .

:Percentage a owl:NamedIndividual, :ReportedValueType ;
    rdfs:label "Percentage"@en .

:Rank a owl:NamedIndividual, :ReportedValueType ;
    rdfs:label "Rank"@en ;
    rdfs:comment "A Rank is always defined as a number between 0 and 10. Other rankings should be mapped up or down to 0-10."@en .

:RawValue a owl:NamedIndividual, :ReportedValueType ;
    rdfs:label "Raw Value"@en .

:SmallDecrease a owl:NamedIndividual, :SeriesTrend ;
    rdfs:label "Small Decrease"@en .

:SmallIncrease a owl:NamedIndividual, :SeriesTrend ;
    rdfs:label "Small Increase"@en .

:TextEnum a owl:NamedIndividual, :ReportedValueType ;
    rdfs:label "Text-based enumerated value"@en .

_:diff1 rdf:type owl:AllDifferent ; 
    owl:members ( :Average :Count :Index :Percentage :Rank :RawValue :TextEnum 
                  :LargeDecrease :LargeIncrease :NoChange :Outlier :SmallDecrease :SmallIncrease ) .
