@prefix : <http://dig.isi.edu/ontologies/dig/> .
@prefix diga: <http://dig.isi.edu/ontologies/dig-annotation/> .
@prefix dc: <http://purl.org/dc/elements/1.1/> .
@prefix dcterms: <http://purl.org/dc/terms/> .
@prefix owl: <http://www.w3.org/2002/07/owl#> .
@prefix rdf: <http://www.w3.org/1999/02/22-rdf-syntax-ns#> .
@prefix xml: <http://www.w3.org/XML/1998/namespace> .
@prefix xsd: <http://www.w3.org/2001/XMLSchema#> .
@prefix rdfs: <http://www.w3.org/2000/01/rdf-schema#> .
@prefix skos: <http://www.w3.org/2004/02/skos/core#> .
@prefix crm: <http://www.cidoc-crm.org/cidoc-crm/> .
@prefix schema: <http://schema.org/> .

###
### This file specifies two ontologies:
### - :diga <http://dig.isi.edu/ontologies/dig-annotation/> 
###   an ontology to annotate other ontologies with information useful to dig
### - : <http://dig.isi.edu/ontologies/dig/>
###   a default generic ontology, useful for multiple applications. Users may use other ontologies.
###

diga:icon_name a owl:DatatypeProperty ;
    rdfs:label "icon name" ;
    skos:definition """Specifies the name of an icon that a user interface may display when showing values of a property or class in the user interface.""" ;
    schema:domainIncludes owl:ObjectProperty, owl:DatatypeProperty, owl:Class ;
    schema:rangeIncludes xsd:string ;
    .

diga:icon_color a owl:DatatypeProperty ;
    rdfs:label "icon color" ;
    skos:definition """Specifies the color of an icon that a user interface may display when showing values of a property or class in the user interface.""" ;
    schema:domainIncludes owl:ObjectProperty, owl:DatatypeProperty, owl:Class ;
    schema:rangeIncludes xsd:string ;
    .

diga:crm_equivalent a owl:ObjectProperty ;
    rdfs:label "CRM equivalent" ;
    skos:definition """Specifies an equivalent class or property in the CRM ontology.""" ;
    schema:domainIncludes owl:ObjectProperty, owl:DatatypeProperty, owl:Class ;
    schema:rangeIncludes owl:ObjectProperty, owl:DatatypeProperty, owl:Class ;
    .


###
### CRM classes excluded from this ontology:
#
# Primitive types not included as they are not necessary
# E59_Primitive Value
# E60_Number
# E61_Time Primitive
# E62_String

# E14_Condition_Assessment
# E15 Identifier Assignment
# E17 Type Assignment
# E34_Inscription
# E78_Collection: the meaning is specific to museum collection. TODO: probably need a general Collection class for physical objects
# E83 Type Creation
# E87 Curation Activity
# E81 Transformation
# E35_Title: seems unecessary in our context as we don't have special properties to attach to titles.
# E36_Visual Item: the purppose of this class seems to be to be a superclass of Mark and Image. As we don't have Mark, we don't need the superclass.
# E37_Mark
# E34_Inscription
# E44_Place Appellation: not used as there is also Place_Name and the distinction is too subtle.
# E46_Section Definition: too specific to cultural heritage documentation.
# E75_Conceptual Object Appellation: it seems to Pedro that one can use Identifier or Name as one example given in the CRM doc is “ISBN 3-7913-1418-1”
# E89_Propositional Object: The distinction between Conceptual_Object and Propositional_Object is very subtle, so we are not including Propositional_Object in this ontology.


# E1_CRM_Entity
:Entity a owl:Class ;
    rdfs:label "Entity" ;
    skos:definition """Everything that can be described, similar to owl:Thing.""" ;
    diga:crm_equivalent crm:E1_CRM_Entity ;
    .

# E55_Type
:Type a owl:Class ;
    owl:subclass :Conceptual_Object ;
    rdfs:label "Type" ;
    skos:definition """Comprises concepts denoted by terms from thesauri and controlled vocabularies used to characterize and classify instances of CRM classes. Instances of E55 Type represent concepts.""" ;
    skos:note """In addition to the properties defined in this ontology with domain :Type, the expectation is that they have a rdfs:label; ideally skos properties such as skos:prefLabel/altLabel and documentary properties such as skos:note/definition/example.""" ;
    diga:crm_equivalent crm:E55_Type ;
    .



:Collection a owl:Class ;
    rdfs:label "Collection" ;
    skos:definition """A collection of something. This class can only have properties which belong to the collection itself not the properties of the elements in it.""" ;
    skos:note """""" ;
    .

 # S9 Property Type
:Property_Type a owl:Class ;
    rdfs:label "Property Type" ;
    skos:definition """When modeling measurements, one creates a :Measurement event, and one needs to record the value measures together with its units (:Dimension), the object that was measured (:measured), and the property of the object that we are measuring (:observed_property_type), e.g., the width, or height, or price, or production level, etc. It is possible that all these properties are not defined as RDF properties in an ontology, e.g., :price is not in the ontology. The idea of :Property_Type is to create controlled vocabularies of properties one can observe, withut requiring that these properties be defined as RDF properties, i.e., the observed properties are data (instances of :Property_Type), so new ones can be added without extending the ontology.""" ;
    skos:definition """Comprises types of properties. Typically, instances of S9 Property Type would be aken from an ontology or terminological system. In particular, instances of this class can be used to describe in a parametric way what kind of properties the values in scientific data sets are about. By virtue of such descriptions, numeric data can be interpreted as sets of propositions in terms of a formal ontology, such as “concentration of nitrate”, observed in the ground water from a certain borehole.""" ;
    owl:subClassOf :Type ;
    diga:crm_equivalent crm:S9_Property_Type ;
    .

# E2_Temporal_Entity
:Temporal_Entity a owl:Class ;
    rdfs:label "Temporal Entity" ;
    skos:definition """Phenomena that happens over time, incuding :Event and :Condition_State.""" ;
    skos:note """This is an abstract class used as domain of temporal properties that apply to :Event and :Condition_State.""" ;
    rdfs:subClassOf :Entity ;
    diga:crm_equivalent crm:E2_Temporal_Entity ;
    :common_properties :title, :description, :identifier ;
    .

:Condition_State a owl:Class ;
    rdfs:label "Condition State" ;
    skos:definition """The states of objects characterised by a certain condition over a time-span.""" ;
    skos:note """For example, being dead, or being destroyed are states that may be caused by an event.""" ;
    rdfs:subClassOf :Temporal_Entity ;
    diga:crm_equivalent crm:E3_Condition_State ;
    .

:Event a owl:Class ;
    rdfs:label "Event" ;
    skos:definition """An event that may happen or has happened in the world.""" ;
    rdfs:subClassOf :Temporal_Entity ;
    diga:crm_equivalent crm:E5_Event ;
    .

:Activity a owl:Class ;
    rdfs:label "Activity" ;
    skos:definition """Comprises actions intentionally carried out by instances of E39 Actor that result in changes of state in the world. The difference with :Event is that events may just "happen" while :Activity implies that an :Actor made them happen.""" ;
    rdfs:subClassOf :Event ;
    diga:crm_equivalent crm:E7_Activity ;
    .

:Acquisition a owl:Class ;
    rdfs:label "Acquisition" ;
    skos:definition """Comprises transfers of legal ownership from one or more instances of E39 Actor to one or more other instances of E39 Actor.""" ;
    rdfs:subClassOf :Activity ;
    diga:crm_equivalent crm:E8_Acquisition ;
    .

:Move a owl:Class ;
    rdfs:label "Move" ;
    skos:definition """Comprises changes of the physical location of the instances of E19 Physical Object.""" ;
    rdfs:subClassOf :Activity ;
    diga:crm_equivalent crm:E9_Move ;
    .

:Transfer_Of_Custody a owl:Class ;
    rdfs:label "Transfer of Custody" ;
    skos:definition """Comprises transfers of physical custody of objects between instances of E39 Actor.""" ;
    rdfs:subClassOf :Activity ;
    diga:crm_equivalent crm:E10_Transfer_Of_Custody ;
    .

:Modification a owl:Class ;
    rdfs:label "Modification" ;
    skos:definition """Comprises all instances of E7 Activity that create, alter or change E24 Physical Man-Made Thing.""" ;
    skos:note """Since the distinction between modification and production is not always clear, modification is regarded as the more generally applicable concept. This implies that some items may be consumed or destroyed in a Modification, and that others may be produced as a result of it. An event should also be documented using E81 Transformation if it results in the destruction of one or more objects and the simultaneous production of others using parts or material from the originals. In this case, the new items have separate identities.""" ;
    rdfs:subClassOf :Activity ;
    diga:crm_equivalent crm:E11_Modification ;
    .

:Production a owl:Class ;
    rdfs:label "Production" ;
    skos:definition """Comprises activities that are designed to, and succeed in, creating one or more new items.""" ;
    rdfs:subClassOf :Modification ;
    diga:crm_equivalent crm:E12_Production ;
    .

:Part_Addition a owl:Class ;
    rdfs:label "Part Addition" ;
    skos:definition """Comprises activities that result in an instance of E24 Physical Man-Made Thing being increased, enlarged or augmented by the addition of a part.""" ;
    rdfs:subClassOf :Modification ;
    diga:crm_equivalent crm:E79_Part_Addition ;
    .

:Part_Removal a owl:Class ;
    rdfs:label "Part Removal" ;
    skos:definition """Comprises the activities that result in an instance of E18 Physical Thing being decreased by the removal of a part.""" ;
    rdfs:subClassOf :Modification ;
    diga:crm_equivalent crm:E80_Part_Removal ;
    .

:Attribute_Assignment a owl:Class ;
    rdfs:label "Attribute Assignment" ;
    skos:definition """Comprises the actions of making assertions about properties of an object or any relation between two items or concepts.""" ;
    skos:note """In particular, the class describes the actions of people making propositions and statements, e.g. the person and date when a condition statement was made, an identifier was assigned, an object was measured, etc.""" ;
    rdfs:subClassOf :Activity ;
    diga:crm_equivalent crm:E13_Attribute_Assignment ;
    .

:Measurement a owl:Class ;
    rdfs:label "Measurement" ;
    skos:definition """Describes an entity being measured and an observed dimension.""" ;
    skos:note """:Measurement is a subclass of event, so it is possible to record additional roles such as time when the measurement was made, who made it, where it was made, etc.""" ;
    skos:note """Examples: Joe's weight is 150 lbs, price of oil is $60""" ;
    rdfs:subClassOf :Attribute_Assignment ;
    diga:crm_equivalent crm:E16_Measurement ;
    :common_properties :observed_dimension, :measured ;
    .

:Creation a owl:Class ;
    rdfs:label "Creation" ;
    skos:definition """Comprises events that result in the creation of conceptual items or immaterial products, such as legends, poems, texts, music, images, movies, laws, types etc.""" ;
    skos:note """Examples: the framing of the U.S. Constitution, the drafting of U.N. resolution 1441""" ;
    rdfs:subClassOf :Activity ;
    diga:crm_equivalent crm:E65_Creation ;
    .

:Formation a owl:Class ;
    rdfs:label "Formation" ;
    skos:definition """Comprises events that result in the formation of a formal or informal E74 Group of people, such as a club, society, association, corporation or nation.""" ;
    skos:note """The formation of an instance of E74 Group does not mean that the group is populated with members at the time of formation. In order to express the joining of members at the time of formation, the respective activity should be simultaneously an instance of both E66 Formation and E85 Joining.""" ;
    rdfs:subClassOf :Activity, :Beginning_Of_Existence ;
    diga:crm_equivalent crm:E66_Formation ;
    .

:Joining a owl:Class ;
    rdfs:label "Joining" ;
    skos:definition """comprises the activities that result in an instance of E39 Actor becoming a member of an instance of E74 Group. This class does not imply initiative by either party.""" ;
    skos:note """Typical scenarios include becoming a member of a social organisation, becoming employee of a company, marriage, the adoption of a child by a family and the inauguration of somebody into an official position.""" ;
    rdfs:subClassOf :Activity ;
    diga:crm_equivalent crm:E85_Joining ;
    .

:Leaving a owl:Class ;
    rdfs:label "Leaving" ;
    skos:definition """Comprises the activities that result in an instance of E39 Actor to be disassociated from an instance of E74 Group. This class does not imply initiative by either party.""" ;
    skos:note """Typical scenarios include the termination of membership in a social organisation, ending the employment at a company, divorce, and the end of tenure of somebody in an official position.""" ;
    rdfs:subClassOf :Activity ;
    diga:crm_equivalent crm:E86_Leaving ;
    .

:Beginning_Of_Existence a owl:Class ;
    rdfs:label "Beginning of Existence" ;
    skos:definition """Comprises events that bring into existence any E77 Persistent Item.""" ;
    skos:note """Examples, the birth of my child; the birth of Snoopy, my dog; the calving of the iceberg that sank the Titanic; the construction of the Eiffel Tower""" ;
    rdfs:subClassOf :Event ;
    diga:crm_equivalent crm:E63_Beginning_Of_Existence ;
    .

:Birth a owl:Class ;
    rdfs:label "Birth" ;
    skos:definition """Comprises the births of human beings. E63 Beginning of Existence comprises the coming into life of any living beings.""" ;
    rdfs:subClassOf :Beginning_Of_Existence ;
    diga:crm_equivalent crm:E67_Birth ;
    .

:End_Of_Existence a owl:Class ;
    rdfs:label "End of Existence" ;
    skos:definition """Comprises events that end the existence of any E77 Persistent Item.""" ;
    rdfs:subClassOf :Event ;
    diga:crm_equivalent crm:E64_End_Of_Existence ;
    .

:Destruction a owl:Class ;
    rdfs:label "Destruction" ;
    skos:definition """Comprises events that destroy one or more instances of E18 Physical Thing such that they lose their identity as the subjects of documentation.""" ;
    rdfs:subClassOf :End_Of_Existence ;
    diga:crm_equivalent crm:E6_Destruction ;
    .

:Dissolution a owl:Class ;
    rdfs:label "Dissolution" ;
    skos:definition """Comprises the events that result in the formal or informal termination of an E74 Group of people.""" ;
    rdfs:subClassOf :End_Of_Existence ;
    diga:crm_equivalent crm:E68_Dissolution ;
    .

:Death a owl:Class ;
    rdfs:label "Death" ;
    skos:definition """Comprises the deaths of human beings.""" ;
    rdfs:subClassOf :End_Of_Existence ;
    diga:crm_equivalent crm:E69_Death ;
    .

:Persistent_Item a owl:Class ;
    rdfs:label "Persistent Item" ;
    skos:definition """Comprises items that have a persistent identity.""" ;
    skos:note """This is an abstract class to tie together actors and things.""" ;
    rdfs:subClassOf :Entity ;
    diga:crm_equivalent crm:E77_Persistent_Item ;
    .

:Thing a owl:Class ;
    rdfs:label "Thing" ;
    skos:definition """Comprises usable discrete, identifiable, instances of E77 Persistent Item that are documented as single units.""" ;
    skos:note """They can be either intellectual products or physical things, and are characterized by relative stability. They may for instance either have a solid physical form, an electronic encoding, or they may be logical concept or structure.""" ;
    rdfs:subClassOf :Persistent_Item ;
    diga:crm_equivalent crm:E70_Thing ;
    .

:Legal_Object a owl:Class ;
    rdfs:label "Legal Object" ;
    skos:definition """Comprises usable discrete, identifiable, instances of E77 Persistent Item that are documented as single units.""" ;
    skos:note """They can be either intellectual products or physical things, and are characterized by relative stability. They may for instance either have a solid physical form, an electronic encoding, or they may be logical concept or structure.""" ;
    rdfs:subClassOf :Thing ;
    diga:crm_equivalent crm:E72_Legal_Object ;
    .

:Physical_Thing a owl:Class ;
    rdfs:label "Physical Thing" ;
    skos:definition """Comprises all persistent physical items with a relatively stable form, man-made or natural.""" ;
    skos:note """Depending on the existence of natural boundaries of such things, the CRM distinguishes the instances of E19 Physical Object from instances of E26 Physical Feature, such as holes, rivers, pieces of land etc. Most instances of E19 Physical Object can be moved (if not too heavy), whereas features are integral to the surrounding matter.""" ;
    rdfs:subClassOf :Legal_Object ;
    diga:crm_equivalent crm:E18_Physical_Thing ;
    .

:Physical_Object a owl:Class ;
    rdfs:label "Physical_Object" ;
    skos:definition """A thing in the world, e.g., buildings, trees, persons, but not ideas.""" ;
    rdfs:subClassOf :Physical_Thing ;
    diga:crm_equivalent crm:E19_Physical_Object ;
    .

:Biological_Object a owl:Class ;
    rdfs:label "Biological Object" ;
    skos:definition """Comprises individual items of a material nature, which live, have lived or are natural products of or from living organisms.""" ;
    rdfs:subClassOf :Physical_Thing ;
    diga:crm_equivalent crm:E20_Biological_Object ;
    .

:Person a owl:Class ;
    rdfs:label "Group" ;
    skos:definition """A specific person in the world, it can be specific, such as a Barack Obama, or unspecific, such as a child.""" ;
    rdfs:subClassOf :Actor, :Biological_Object ;
    diga:crm_equivalent crm:E21_Person ; 
    :common_properties :label, :title, :religion ;
    .

# E22 Man-Made Object
:Man_Made_Object a owl:Class ;
    rdfs:label "Man-Made Thing" ;
    skos:definition """Comprises physical objects purposely created by human activity.""" ;
    rdfs:subClassOf :Physical_Object, :Physical_Man_Made_Thing ;
    diga:crm_equivalent crm:E22_Man-Made_Object ;
    .

# E84_Information Carrier
:Information_Carrier a owl:Class ;
    rdfs:label "Information Carrier" ;
    skos:definition """Comprises all instances of E22 Man-Made Object that are explicitly designed to act as persistent physical carriers for instances of E73 Information Object.""" ;
    skos:note """Examples: the Rosetta Stone; my paperback copy of Crime & Punishment; the computer disk in my laptop.""" ; 
    rdfs:subClassOf :Man_Made_Object ;
    diga:crm_equivalent crm:E84_Information_Carrier ;
    .

# E26_Physical Feature: 
:Physical_Feature a owl:Class ;
    rdfs:label "Physical Feature" ;
    skos:definition """Comprises identifiable features that are physically attached in an integral way to particular physical objects.""" ;
    skos:note """Instances of E26 Physical Feature can be features in a narrower sense, such as scratches, holes, reliefs, surface colours, reflection zones in an opal crystal or a density change in a piece of wood. In the wider sense, they are portions of particular objects with partially imaginary borders, such as the core of the Earth, an area of property on the surface of the Earth, a landscape or the head of a contiguous marble statue. They can be measured and dated, and it is sometimes possible to state who or what is or was responsible for them. They cannot be separated from the carrier object, but a segment of the carrier object may be identified (or sometimes removed) carrying the complete feature.""" ; 
    rdfs:subClassOf :Physical_Thing ;
    diga:crm_equivalent crm:E26_Physical_Feature ;
    .

# E27_Site: 
:Site a owl:Class ;
    rdfs:label "Site" ;
    skos:definition """Comprises pieces of land or sea floor.""" ;
    skos:note """In contrast to the purely geometric notion of E53 Place, this class describes constellations of matter on the surface of the Earth or other celestial body, which can be represented by photographs, paintings and maps.""" ; 
    skos:note """Examples: the Amazon river basin; Knossos ; the Apollo 11 landing site; Heathrow Airport; the submerged harbour of the Minoan settlement of Gournia, Crete.""" ;
    rdfs:subClassOf :Physical_Feature ;
    diga:crm_equivalent crm:E27_Site ;
    .

# E90_Symbolic Object
:Symbolic_Object a owl:Class ;
    rdfs:label "Symbolic Object" ;
    skos:definition """Comprises identifiable symbols and any aggregation of symbols, such as characters, identifiers, traffic signs, emblems, texts, data sets, images, musical scores, multimedia objects, computer program code or mathematical formulae that have an objectively recognizable structure and that are documented as single units.""" ;
    skos:note """It includes sets of signs of any nature, which may serve to designate something, or to communicate some propositional content.""" ;
    skos:note """An instance of E90 Symbolic Object does not depend on a specific physical carrier, which can include human memory, and it can exist on one or more carriers simultaneously. An instance of E90 Symbolic Object may or may not have a specific meaning, for example an arbitrary character string.""" ;
    rdfs:subClassOf :Conceptual_Object, :Legal_Object ;
    diga:crm_equivalent crm:E90_Symbolic_Object ;
    .

# E73_Information Object
:Information_Object a owl:Class ;
    rdfs:label "Information Object" ;
    skos:definition """Comprises identifiable immaterial items, such as a poems, jokes, data sets, images, texts, multimedia objects, procedural prescriptions, computer program code, algorithm or mathematical formulae, that have an objectively recognizable structure and are documented as single units.""" ;
    skos:note """An E73 Information Object does not depend on a specific physical carrier, which can include human memory, and it can exist on one or more carriers simultaneously.""" ;
    skos:note """Instances of E73 Information Object of a linguistic nature should be declared as instances of the E33 Linguistic Object subclass. Instances of E73 Information Object of a documentary nature should be declared as instances of the E31 Document subclass. ideas without a reproducible expression are not instances of E73 Information Object.""" ;
    rdfs:subClassOf :Propositional_Object, :Symbolic_Object ;
    diga:crm_equivalent crm:E73_Information_Object ;
    .
  
# E29_Design or Procedure
:Design_Or_Procedure a owl:Class ;
    rdfs:label "Design or Procedure" ;
    skos:definition """Comprises documented plans for the execution of actions in order to achieve a result of a specific quality, form or contents. In particular it comprises plans for deliberate human activities that may result in the modification or production of instances of E24 Physical Thing.""" ;
    skos:note """Instances of E29 Design or Procedure can be structured in parts and sequences or depend on others. This is modelled using P69 is associated with.""" ;
    skos:note """Designs or procedures can be seen as one of the following: 1. A schema for the activities it describes; 2. A schema of the products that result from their application; 3. An independent intellectual product that may have never been applied, such as Leonardo da Vinci’s famous plans for flying machines.""" ;
    rdfs:subClassOf :Information_Object ;
    diga:crm_equivalent crm:E29_Design_or_Procedure ;
    .

# E31_Document
:Document a owl:Class ;
    rdfs:label "Document" ;
    skos:definition """Comprises identifiable immaterial items that make propositions about reality.""" ;
    skos:note """These propositions may be expressed in text, graphics, images, audiograms, videograms or by other similar means. Documentation databases are regarded as a special case of E31 Document. This class should not be confused with the term “document” in Information Technology, which is compatible with E73 Information Object.""" ;
    rdfs:subClassOf :Information_Object ;
    diga:crm_equivalent crm:E31_Document ;
    .

# E32_Authority Document
:Authority_Document a owl:Class ;
    rdfs:label "Authority Document" ;
    skos:definition """Comprises encyclopaedia, thesauri, authority lists and other documents that define terminology or conceptual systems for consistent use.""" ;
    rdfs:subClassOf :Document ;
    diga:crm_equivalent crm:E32_Authority_Document ;
    .

# E33_Linguistic Object
:Linguistic_Object a owl:Class ;
    rdfs:label "Linguistic Object" ;
    skos:definition """Comprises identifiable expressions in natural language or languages.""" ;
    skos:note """nstances of E33 Linguistic Object can be expressed in many ways: e.g. as written texts, recorded speech or sign language. However, the CRM treats instances of E33 Linguistic Object independently from the medium or method by which they are expressed. Expressions in formal languages, such as computer code or mathematical formulae, are not treated as instances of E33 Linguistic Object by the CRM (because code is not in natural language). These should be modelled as instances of E73 Information Object. The text of an instance of E33 Linguistic Object can be documented in a note by P3 has note: E62 String.""" ;
    rdfs:subClassOf :Information_Object ;
    diga:crm_equivalent crm:E33_Linguistic_Object ;
    .

# E38_Image# 
:Image a owl:Class ;
    rdfs:label "Image" ;
    skos:definition """Comprises distributions of form, tone and colour that may be found on surfaces such as photos, paintings, prints and sculptures or directly on electronic media.""" ;
    skos:note """To-Do: explain how to record the url or location of an image, it's mime type, etc.""" ;
    rdfs:subClassOf :Information_Object ;
    diga:crm_equivalent crm:E38_Image ;
    .

# E41_Appellation
:Name a owl:Class ;
    rdfs:label "Name" ;
    skos:definition """The name of an instance of a class.""" ;
    skos:note """The main reason to define a Name class is that in addition to the label, it can have other properties such as type. The type field can be used to distinguish different types of names. For example, given or family names for people, and differen types of identifiers such as social security, doi, etc.""" ;
    rdfs:subClassOf :Information_Object ;
    diga:crm_equivalent crm:E41_Appellation ;
    .

# E42_Identifier
:Identifier a owl:Class ;
    rdfs:label "Identifier" ;
    skos:definition """Comprises strings or codes assigned to instances of E1 CRM Entity in order to identify them uniquely and permanently within the context of one or more organisations. Such codes are often known as inventory numbers, registration codes, etc. and are typically composed of alphanumeric sequences.""" ;
    skos:note """While there are no properties whose domain is Identifier, and thus are indistinguishable from names, the expectation is that all Identifiers will have a type, while names often do not.""" ;
    rdfs:subClassOf :Name ;
    diga:crm_equivalent crm:E42_Identifier ;
    .

# E48_Place Name
:Place_Name a owl:Class ;
    rdfs:label "Place Name" ;
    skos:definition """Comprises any sort of name characteristically used to refer to an E53 Place.""" ;
    skos:note """This class corresponds to E44_Place_Appellation and not to E48_Place_Name, as we don't have a corresponding class to E48_Place_Name.""" ;
    rdfs:subClassOf :Name ;
    diga:crm_equivalent crm:E44_Place_Appellation ;
    .

# E45_Address
:Address a owl:Class ;
    rdfs:label "Address" ;
    skos:definition """Comprises names to identify places, such as postal addresses used for mailing.""" ;
    skos:note """Postal Office Boxes are a form of address that identifies a contact point for an actor without necessarily identifying a place.""" ;
    skos:note """To Do: define simiarly to schema:Address.""" ;
    rdfs:subClassOf :Place_Name, :Contact_Point ;
    diga:crm_equivalent crm:E45_Address ;
    .

# E47_Spatial Coordinates
:Spatial_Coordinates a owl:Class ;
    rdfs:label "Spatial Coordinates" ;
    skos:definition """Comprises the textual or numeric information required to locate specific instances of E53 Place.  Coordinates are not restricted to longitude, latitude and altitude. Any regular system of reference that maps onto an E19 Physical Object can be used to generate coordinates.""" ;
    skos:note """One could argue that an :Address should be a subclass of Spatial_Coordinates, as it locates a place.  The distinction is one of convention.""" ;
    skos:note """To Do: define properties for recording latitude, longitude, etc.""" ;
    rdfs:subClassOf :Place_Name ;
    diga:crm_equivalent crm:E47_Spatial_Coordinates ;
    .

# E49_Time Appellation
:Time_Span_Name a owl:Class ;
    rdfs:label "Time Span Name" ;
    skos:definition """comprises all forms of names or codes, such as historical periods, and dates, which are characteristically used to refer to a specific E52 Time-Span.""" ;
    skos:note """The names vary in precision, and are not required to be easy to parse by software. For example "before Christ", "after the superbowl", “1215 Hegira” [a date in the Islamic calendar].""" ;
    rdfs:subClassOf :Name ;
    diga:crm_equivalent crm:E49_Time_Appellation ;
    .

# E50_Date
:Date a owl:Class ;
    rdfs:label "Date" ;
    skos:definition """Comprises specific forms of Time_Span_Name (E49 Time Appellation).""" ;
    skos:note """Dates may vary in precision, e.g., unix epochs or years.""" ;
    skos:note """When a time span can be identified using a computer parsable name, then an instance of Date should be used. When a time span cannot be parsed then a Time_Span_Name should be used.""" ;
    rdfs:subClassOf :Time_Span_Name ;
    diga:crm_equivalent crm:E50_Date ;
    .

# E82_Actor Appellation
:Actor_Name a owl:Class ;
    rdfs:label "Date" ;
    skos:definition """Comprises names of actors, such as people, organizations, groups.""" ;
    rdfs:subClassOf :Name ;
    diga:crm_equivalent crm:E82_Actor_Appellation ;
    .

# E51_Contact Point
:Contact_Point a owl:Class ;
    rdfs:label "Contact Point" ;
    skos:definition """Comprises identifiers employed, or understood, by communication services to direct communications to an instance of E39 Actor. These include E-mail addresses, telephone numbers, post office boxes, Fax numbers, URLs etc. Most postal addresses can be considered both as instances of E44 Place Appellation and E51 Contact Point. In such cases the subclass E45 Address should be used.""" ;
    skos:note """CIDOC CRM considers URLs as contact points according to the following argument: "URLs are addresses used by machines to access another machine through an http request. Since the accessed machine acts on behalf of the E39 Actor providing the machine, URLs are considered as instances of E51 Contact Point to that E39 Actor." We consider URLs as identifiers of resources on the web.""" ;
    skos:note """To Do: either define subclasses for phone, email, etc. or controlled vocabulary to use in type, e.g. type = :telephone.""" ;
    rdfs:subClassOf :Name ;
    diga:crm_equivalent crm:E51_Contact_Point ;
    .

# E71_Man-Made Thing
:Man_Made_Thing a owl:Class ;
    rdfs:label "Man-Made Thing" ;
    skos:definition """Comprises discrete, identifiable man-made items that are documented as single units. These items are either intellectual products or man-made physical things, and are characterized by relative stability. They may for instance have a solid physical form, an electronic encoding, or they may be logical concepts or structures.""" ;
    skos:note """Beethoven’s 5th Symphony, Michelangelo’s David, Einstein’s Theory of General Relativity, the Linux operating system, the Empire State building, a chair.""" ;
    rdfs:subClassOf :Entity, :Thing;
    diga:crm_equivalent crm:E71_Man-Made_Thing ;
    .

# E24_Physical Man-Made Thing
:Physical_Man_Made_Thing a owl:Class ;
    rdfs:label "Physical Man-Made Thing" ;
    skos:definition """Comprises man-made objects, such as a swords, and man-made features, such as rock art. No assumptions are made as to the extent of modification required to justify regarding an object as man-made.""" ;
    skos:note """The distinction between Thing and Object is subtle. A car is both a thing and an object, while a carving on a rock is a thing, but not an obejct.""" ;
    rdfs:subClassOf :Physical_Thing, :Man_Made_Thing ;
    diga:crm_equivalent crm:E24_Physical_Man-Made_Thing ;
    .

# E22_Man-Made Object
:Man_Made_Object a owl:Class ;
    rdfs:label "Man-Made Object" ;
    skos:definition """Comprises physical objects purposely created by human activity.""" ;
    skos:note """No assumptions are made as to the extent of modification required to justify regarding an object as man-made. For example, an inscribed piece of rock or a preserved butterfly are both regarded as instances of E22 Man-Made Object. The inscription on the rock is not an object but it is a man made thing.""" ;
    rdfs:subClassOf :Physical_Object, :Physical_Man_Made_Thing ;
    diga:crm_equivalent crm:E22_Man-Made_Object ;
    .

# E84_Information Carrier
:Information_Carrier a owl:Class ;
    rdfs:label "Information Carrier" ;
    skos:definition """Comprises all instances of E22 Man-Made Object that are explicitly designed to act as persistent physical carriers for instances of E73 Information Object.""" ;
    skos:note """This allows a relationship to be asserted between an E19 Physical Object and its immaterial information contents. An E84 Information Carrier may or may not contain information, e.g., a diskette. Note that any E18 Physical Thing may carry information, such as an E34 Inscription. However, unless it was specifically designed for this purpose, it is not an Information Carrier. Therefore the property P128 carries (is carried by) applies to E18 Physical Thing in general.""" ;
    rdfs:subClassOf :Man_Made_Object ;
    diga:crm_equivalent crm:E84_Information_Carrier ;
    .

# E25_Man-Made Feature
:Man_Made_Feature a owl:Class ;
    rdfs:label "Man-Made Feature" ;
    skos:definition """Comprises physical features that are purposely created by human activity, such as scratches, artificial caves, artificial water channels, etc.""" ;
    skos:note """No assumptions are made as to the extent of modification required to justify regarding a feature as man-made. For example, rock art or even “cup and ring” carvings on bedrock a regarded as types of E25 Man-Made Feature.""" ;
    rdfs:subClassOf :Physical_Man_Made_Thing, :Physical_Feature ;
    diga:crm_equivalent crm:E25_Man-Made-Feature ;
    .

# E28_Conceptual Object
:Conceptual_Object a owl:Class ;
    rdfs:label "Conceptual Object" ;
    skos:definition """Comprises non-material products of our minds and other human produced data that have become objects of a discourse about their identity, circumstances of creation or historical implication. The production of such information may have been supported by the use of technical devices such as cameras or computers.""" ;
    skos:note """Characteristically, instances of this class are created, invented or thought by someone, and then may be documented or communicated between persons. Instances of E28 Conceptual Object have the ability to exist on more than one particular carrier at the same time, such as paper, electronic signals, marks, audio media, paintings, photos, human memories, etc.""" ;
    skos:note """They cannot be destroyed. They exist as long as they can be found on at least one carrier or in at least one human memory. Their existence ends when the last carrier and the last memory are lost.""" ;
    skos:note """The distinction between Conceptual_Object and Propositional_Object is very subtle, so we are not including Propositional_Object in this ontology.""" ;
    rdfs:subClassOf :Man_Made_Thing ;
    diga:crm_equivalent crm:E28_Conceptual_Object ;
    .

# E30_Right
:Right a owl:Class ;
    rdfs:label "Right" ;
    skos:definition """Comprises legal privileges concerning material and immaterial things or their derivatives.""" ;
    skos:note """Examples: "copyright held by ISO on ISO/CD", "ownership of the Mona Lisa by the Louvre" """ ;
    rdfs:subClassOf :Conceptual_Object ;
    diga:crm_equivalent crm:E30_Right ;
    .

:Actor a owl:Class ;
    rdfs:label "Actor" ;
    skos:definition """A group, organization, person who have the potential to do actions, e.g., rob a bank, make a public statement.""" ; 
    rdfs:subClassOf :Persistent_Item ;
    diga:crm_equivalent crm:E39_Actor ;
    :common_properties :label, :title, :religion ;
    .

:Group a owl:Class ;
    rdfs:label "Group" ;
    skos:definition """A """ ;
    rdfs:subClassOf :Actor, :Collection ;
    diga:crm_equivalent crm:E74_Group ;
    :common_properties :label, :title ;
    .

:Organization a owl:Class ;
    rdfs:label "Group" ;
    skos:definition """Any type of organizationm, a company, a terrorist group, a government, etc.""" ;
    rdfs:subClassOf :Group ;
    diga:crm_equivalent crm:E40_Legal_Body ;
    :common_properties :label, :title, :religion ;
    .

# E53_Place
:Place a owl:Class ;
    rdfs:label "Place" ;
    skos:definition """Any place at any level of granularity""" ;
    rdfs:subClassOf :Entity ;
    diga:crm_equivalent crm:E53_Place ;
    :common_properties :label, :title, :city, :state, :country, :region, :iso_country_code, :adm1_code ;
    .

# E54_Dimension
:Dimension a owl:Class ;
    rdfs:label "Dimension" ;
    skos:definition """Identifies a value and its unit of measurement.""" ;
    skos:note """Values are specified using :has_value, :value_is_at_least or :value_is_at_most. When the numeric value is unknown, e.g., "a large sum of money", it should be recorded as the :label.""" ;
    skos:note """Examples: currency: $26.00, length: 3.9-4.1 cm, diameter 26 mm, weight 150 lbs""" ;
    rdfs:subClassOf :Entity ;
    diga:crm_equivalent crm:E54_Dimension ;
    .

:Time_Span a owl:Class ;
    rdfs:label "Time Span" ;
    skos:definition """Defines a span of time. Allows for imprecise specification, including natural language text.""" ;
    skos:note """When a :Time_Span is defined using natural language, e.g., "1st half of the XX century" and the information extraction software is unable to make it precise, then the text is used as the :title, and no other information may be present.""" ;
    skos:note """P82 at some time within, and P81 ongoing throughout are specified using :start_date, :start_after_date, :start_before_date, :end_date, :end_after_date, :end_before_date. With these properties it is possible to specify the whole interval without additional objects.""" ;
    skos:note """Suppose we are told that someone was born ins 1998. This can be modelled as a :Time_Span with from 1 Jan 1998 at midnight to midnight of 31 Dec 1998. It can also be modeled by specifying the :start_time 1 Jan 1998 at midnight and a duration of one year. And it can also be modeled using :year 1998.""" ;
    rdfs:subClassOf :Entity ;
    diga:crm_equivalent crm:E52_Time-Span ;
    .

:Religion a owl:Class ;
    rdfs:label "Religion" ;
    skos:definition """Identifies a religion in the world.""" ;
    skos:note """To Do: need to define properties that associate religions with Actors.""" ;
    rdfs:subClassOf :Type ;
    .

:Money a owl:Class ;
    rdfs:label "Money" ;
    skos:definition """Identifies an amount of money in some currency.""" ;
    rdfs:subClassOf :Dimension ;
    .


###
### Controlled Vocabularies
###


# E56_Language
:Language a owl:Class ;
    rdfs:label "Language" ;
    skos:definition """Comprises the natural languages.""" ;
    rdfs:subClassOf :Type ;
    diga:crm_equivalent crm:E56_Language ;
    .

# E57_Material
:Material a owl:Class ;
    rdfs:label "Material" ;
    skos:definition """Comprises the concepts of materials.""" ;
    rdfs:subClassOf :Type ;
    diga:crm_equivalent crm:E57_Material ;
    .

# E58_Measurement_Unit
:Measurement_Unit a owl:Class ;
    rdfs:label "Measurement Unit" ;
    skos:definition """Comprises the types of measurement units: feet, inches, centimetres, litres, lumens, etc.""" ;
    rdfs:subClassOf :Type ;
    diga:crm_equivalent crm:E58_Measurement_Unit ;
    .

:Country a owl:Class ;
    rdfs:label "Country" ;
    skos:definition """The set of countries, expressed in a controlled vocabulary.""" ;
    rdfs:subClassOf :Type ;
    .

:Ethnic_Group a owl:Class ;
    rdfs:label "Ethnic Group" ;
    skos:definition """The set of ethnic groups of the world expressed in a controlled vocabulary.""" ;
    rdfs:subClassOf :Type ;
    .

:Modality a owl:Class ;
    rdfs:label "Modality" ;
    skos:definition """A knowledge graph can record events that happened, hypothetical events, events expected to happen in the future, etc. :Modality is a controlled vocabulary for this type of information about an event.""" ;
    skos:note """CauseEx used :has_tense, with values :past, :present and :future, I don't agree with that definition.""" ;
    rdfs:subClassOf :Type ;
    .

:Human_Condition a owl:Class ;
    rdfs:label "Human Condition" ;
    skos:definition """The set of human conditions, such as being poor, rich, injured, dead, displaced, etc.""" ;
    rdfs:subClassOf :Type ;
    .


#################################################################################################
#
# Properties 
#
#################################################################################################

# P3 has note: skos:note should be used instead.

# P1 is identified by (identifies)
:is_identified_by a owl:ObjectProperty ;
    rdfs:label "is identified by" ;
    skos:definition """Describes the naming or identification of any real world item by a name or any other identifier.""" ;
    schema:domainIncludes :Entity ;
    schema:rangeIncludes :Name ;
    diga:crm_equivalent crm:P1_is_identified_by ;
    .

# PP2 has type (is type of)
:has_type a owl:ObjectProperty ;
    rdfs:label "has type" ;
    skos:definition """allows sub typing of CRM entities - a form of specialisation – through the use of a terminological hierarchy, or thesaurus..""" ;
    schema:domainIncludes :Entity ;
    schema:rangeIncludes :Type ;
    diga:crm_equivalent crm:P2_has_type ;
    .

# P4 has time-span (is time-span of)
:has_time_span a owl:ObjectProperty ;
    rdfs:label "has time-span" ;
    skos:definition """The time interval when the :E2_Temporal_Entity happened.""" ;
    skos:note """The related E52 Time-Span is understood as the real Time-Span during which the phenomena were active, which make up the temporal entity instance. It does not convey any other meaning than a positioning on the “time-line” of chronology. The Time-Span in turn is approximated by a set of dates (E61 Time Primitive). A temporal entity can have in reality only one Time-Span, but there may exist alternative opinions about it, which we would express by assigning multiple Time-Spans. Related temporal entities may share a Time-Span. Time-Spans may have completely unknown dates but other descriptions by which we can infer knowledge.""";
    schema:domainIncludes :Temporal_Entity ;
    schema:rangeIncludes :Time_Span ;
    diga:crm_equivalent crm:P4_has_time-span ;
    .

# P5 consists of (forms part of)
:consists_of a owl:ObjectProperty ;
    rdfs:label "consists of" ;
    skos:definition """Describes the decomposition of an E3 Condition State into discrete, subsidiary states.""" ;
    skos:example """The Condition State of the ruined Parthenon (E3) consists of the bombarded state after the explosion of a Venetian shell in 1687 (E3)""" ;
    schema:domainIncludes :Condition_State ;
    schema:rangeIncludes :Condition_State ;
    diga:crm_equivalent crm:P5_consists_of ;
    .

# P7 took place at (witnessed)
:took_place_at a owl:ObjectProperty ;
    rdfs:label "took place at" ;
    skos:definition """Records a :Place associated with a :Temporal_Entity.""" ;
    skos:example """the period “Révolution française” (E4) took place at France (E53)""" ;
    schema:domainIncludes :Event ;
    schema:rangeIncludes :Place ;
    diga:crm_equivalent crm:P7_took_place_at ;
    .

# P8 took place on or within (witnessed)
:took_place_on_or_within a owl:ObjectProperty ;
    rdfs:label "took place on or within" ;
    skos:definition """Describes the location of Temporal_Entity with respect to :Physical_Object, e.g., an event that took place inside a building, and perhaps we don't know where the building is.""" ;
    skos:example """the coronation of Queen Elizabeth II (E7) took place on or within Westminster Abbey (E19)""" ;
    schema:domainIncludes :Temporal_Entity ;
    schema:rangeIncludes :Physical_Object ;
    diga:crm_equivalent crm:P8_took_place_on_or_within ;
    .

# P9 consists of (forms part of)
:period_consists_of a owl:ObjectProperty ;
    rdfs:label "period consists of" ;
    skos:definition """Describes the decomposition of an instance of E4 Period into discrete, subsidiary periods.""" ;
    skos:note """An event consisting of sub-events would be described having period_consists_of sub-events.""" ;
    schema:domainIncludes :Period ;
    schema:rangeIncludes :Period ;
    diga:crm_equivalent crm:P9_consists_of ;
    .

# P10 falls within (contains)
:falls_within a owl:ObjectProperty ;
    rdfs:label "falls within" ;
    skos:definition """Describes an instance of E4 Period, which falls within the E53 Place and E52 Time-Span of another.""" ;
    skos:note """Potentially unrelated events that fall withing a place and time span would be related as falls_within. If somehow they are part of a larger event then period_consistes_of would be used to link the parent event to the sub-events.""" ;
    schema:domainIncludes :Period ;
    schema:rangeIncludes :Period ;
    diga:crm_equivalent crm:P9_consists_of ;
    .

# P11 had participant (participated in)
:had_participant a owl:ObjectProperty ;
    rdfs:label "had participant" ;
    skos:definition """An :Actor who had an active or passive participation in an Event.""" ;
    skos:note """:Actors have the potential to play active roles in events, and but they can also play passive roles, such as being an observer or a victim.""" ;
    schema:domainIncludes :Event ;
    schema:rangeIncludes :Actor ;
    owl:subPropertyOf :occurred_in_the_presence_of ;
    diga:crm_equivalent crm:P11:had_participant ;
    .

# P12 occurred in the presence of (was present at)
:occurred_in_the_presence_of a owl:ObjectProperty ;
    rdfs:label "occurred in the presence of" ;
    skos:definition """Entities that were present during the event and are somehow relevant to the event, e.g., a car or building destroyed in a bombing, a car that was parked close by, the weapon used, people who witnessed the event.""" ;
    skos:note """This is a general property to model a relationship between an event and an entity. Often a more specific subPropertyOf can be used to model the relationship more precisely.""" ; 
    schema:domainIncludes :Event ;
    schema:rangeIncludes :Persistent_Item ;
    diga:crm_equivalent crm:P12_occurred_in_the_presence_of ;
    .

# P13 destroyed (was destroyed by)
:destroyed a owl:ObjectProperty ;
    rdfs:label "destroyed" ;
    skos:definition """A :Physical_Object that is physically destroyed in an event.""" ;
    skos:note """Typically applies to things such as buildings, animals, but technically also applies to people as they are :Physical_Object. """ ;
    skos:note """Destroying the peace between countries would not be modelled as destroyed, but nore generally as took_out_of_existence.""" ;
    schema:rangeIncludes :Physical_Object ;
    owl:subPropertyOf :took_out_of_existence ;
    diga:crm_equivalent crm:P13_destroyed ;
    .

# P14 carried out by (performed)
:carried_out_by a owl:ObjectProperty ;
    rdfs:label "carried out by" ;
    skos:definition """An :Actor that played an active role in an event. :carried_out_by implies causal or legal responsibility.""" ;
    schema:domainIncludes :Activity ;
    schema:rangeIncludes :Actor ;
    owl:subPropertyOf :had_participant ;
    diga:crm_equivalent crm:P14_carried_out_by ;
    .

# P15 was influenced by (influenced)
:was_influenced_by a owl:ObjectProperty ;
    rdfs:label "was influenced by" ;
    skos:definition """A high level property, which captures the relationship between an :Event and anything that may have had some bearing upon it.""" ;
    schema:domainIncludes :Activity ;
    schema:rangeIncludes :Entity ;
    diga:crm_equivalent crm:P15_was_influenced_by ;
    .

# P16 used specific object (was used for)
:used_specific_object a owl:ObjectProperty ;
    rdfs:label "used specific object" ;
    skos:definition """Describes the use of material or immaterial things in a way essential to the performance or the outcome of an :Event.""" ;
    skos:note """It implies that the presence of the object in question was a necessary condition for the action. For example, weapons or bombs used in a violent act.""" ;
    schema:domainIncludes :Activity ;
    schema:rangeIncludes :Thing ;
    owl:subPropertyOf :occurred_in_the_presence_of, :was_influenced_by ;
    diga:crm_equivalent crm:P16_used_specific_object ;
    .

# P17 was motivated by (motivated)
:was_motivated_by a owl:ObjectProperty ;
    rdfs:label "was motivated by" ;
    skos:definition """Describes an item or items that are regarded as a reason for carrying out the :Event.""" ;
    skos:note """For example, the resignation of the chief executive, was motivated by the collapse of SwissAir.""" ;
    schema:domainIncludes :Activity ;
    schema:rangeIncludes :Entity ;
    owl:subPropertyOf :was_influenced_by ;
    diga:crm_equivalent crm:P17_was_motivated_by ;
    .

# P19 was intended use of (was made for):
:was_intended_use_of a owl:ObjectProperty ;
    rdfs:label "was intended use of" ;
    skos:definition """Describes an item or items that are regarded as a reason for carrying out the :Event.""" ;
    skos:note """For example, the resignation of the chief executive, was motivated by the collapse of SwissAir.""" ;
    schema:domainIncludes :Activity ;
    schema:rangeIncludes :Entity ;
    owl:subPropertyOf :used_specific_object ;
    diga:crm_equivalent crm:P19_was_intended_use_of ;
    .

# P93 took out of existence (was taken out of existence by)

# 
:had_specific_purpose a owl:ObjectProperty ;
    rdfs:label "had specific purpose" ;
    skos:definition """Identifies the relationship between a preparatory activity (the subject) and the event it is intended to be preparation for (the object). This includes activities, orders and other organisational actions, taken in preparation for other activities or events.""" ;
    skos:note """The CRM documentation specifies that the preparatory activity must have succeeded. Not clear that this is necessary in our setitng as we can model events that haven't happened, e.g., a plan to do something may include preparatory activities and one hasn't done any of them.""" ;
    skos:note """CRM defines "P21 had general purpose": This may involve activities intended as preparation for some type of activity or event. P21had general purpose (was purpose of) differs from P20 had specific purpose (was purpose of) in that no occurrence of an event is implied as the purpose.""" ;
    schema:domainIncludes :Activity ;
    schema:rangeIncludes :Event ;
    owl:subPropertyOf :used_specific_object ;
    diga:crm_equivalent crm:P20_had_specific_purpose ;
    .

###
### Properties of :Event
###

:had_modality a owl:ObjectProperty ;
    rdfs:label "had_modality" ;
    skos:definition """Records the :Modality of an :Event.""" ;
    schema:domainIncludes :Event ;
    schema:rangeIncludes :Modality ;
    .








:damaged a owl:ObjectProperty ;
    rdfs:label "damaged" ;
    skos:definition """A :Physical_Object that is physically damaged in an event.""" ;
    skos:note """Victims of violent acts who are injured or killed qualify as damage under the current definition of :Physical_Object. If cattle are killed in a violent act, is it damage because victims are :Actor.""" ;
    schema:rangeIncludes :Physical_Object ;
    owl:subPropertyOf :participant ;
    .





:had_provider a owl:ObjectProperty ;
    rdfs:label "had provider" ;
    skos:definition """An :Actor that provided something that was used in an :Event.""" ;
    skos:note """For example, the :Actor who provided a bomb was used in a bombing attack, or provided a password to hack an account, or provided money to help hungry children.""" ;
    schema:domainIncludes :Event ;
    schema:rangeIncludes :Actor ;
    owl:subPropertyOf :carried_out_by ;
    .

:transferred_ownership_to a owl:ObjectProperty ;
    rdfs:label "transferred ownership to" ;
    skos:definition """Identifies an :Actor that acquires the legal ownership of an object as a result of an :Event.""" ;
    skos:note """This property is a sub-property of :carried_out_by, which implies that the :Actor played an active role; the need for the actor to play an active role is debatable.""" ;
    skos:note """The property will typically describe an :Actor purchasing or otherwise acquiring an object from another Actor. However, ownership may also be acquired, without any corresponding loss of ownership by another Actor, through legal fieldwork such as hunting, shooting or fishing.""" ;
    skos:note """Note the renaming of transferred_title_from to transferred_ownership_from.""" ;
    schema:domainIncludes :Event ;
    schema:rangeIncludes :Actor ;
    owl:subPropertyOf :carried_out_by ;
    diga:crm_equivalent crm:P22_transferred_title_to ;
    .

:transferred_ownership_from a owl:ObjectProperty ;
    rdfs:label "transferred ownership from" ;
    skos:definition """Identifies an :Actor that acquires the legal ownership of an object as a result of an :Event.""" ;
    skos:note """Note the renaming of transferred_title_to to transferred_ownership_to.""" ;
    schema:domainIncludes :Event ;
    schema:rangeIncludes :Actor ;
    owl:subPropertyOf :had_provider ;
    diga:crm_equivalent crm:P23_transferred_title_from ;
    .

:transferred_ownership_of a owl:ObjectProperty ;
    rdfs:label "transferred ownership of" ;
    skos:definition """Identifies the items involved in an acquisition :Event.""" ;
    skos:note """CRM defines the domain to be Physical_Object, we have expanded it to include non physical things such as organizations, software, etc.""" ;
    schema:domainIncludes :Event ;
    schema:rangeIncludes :Physical_Object, :Physical_Man_Made_Thing ;
    owl:subPropertyOf :occurred_in_the_presence_of ;
    diga:crm_equivalent crm:P24_transferred_title_of ;
    .

:custody_surrendered_by a owl:ObjectProperty ;
    rdfs:label "custody surrendered by" ;
    skos:definition """Identifies an :Actor who surrenders custody of an item as a result of an :Event.""" ;
    skos:note """This property is a sub-property of :carried_out_by, which implies that the :Actor played an active role; the need for the actor to play an active role is debatable.""" ;
    skos:note """The property will typically describe an :Actor surrendering custody of an object when it is handed over to someone else’s care. On occasion, physical custody may be surrendered involuntarily – through accident, loss or theft.""" ;
    schema:domainIncludes :Event ;
    schema:rangeIncludes :Actor ;
    owl:subPropertyOf :had_provider ;
    diga:crm_equivalent crm:P28_custody_surrendered_by ;
    .

:custody_received_by a owl:ObjectProperty ;
    rdfs:label "custody received by" ;
    skos:definition """identifies the an :Actor who receives custody of an an item as a result of an :Event.""" ;
    skos:note """Typically used for museum objects where an owner transfers custody, but not ownership of an object to a museum.""" ;
    schema:domainIncludes :Event ;
    schema:rangeIncludes :Actor ;
    owl:subPropertyOf :carried_out_by ;
    diga:crm_equivalent crm:P29_custody_received_by ;
    .

:transferred_custody_of a owl:ObjectProperty ;
    rdfs:label "transferred custody of" ;
    skos:definition """Identifies an item or items whose custody is transferred as a result of an :Event.""" ;
    schema:domainIncludes :Event ;
    schema:rangeIncludes :Physical_Object, :Physical_Man_Made_Thing ;
    owl:subPropertyOf :had_participant ;
    diga:crm_equivalent crm:P30_transferred_custody_of ;
    .

:moved a owl:ObjectProperty ;
    rdfs:label "moved" ;
    skos:definition """Identifies a :Physical_Object that is moved during a move :Event.""" ;
    schema:domainIncludes :Event ;
    schema:rangeIncludes :Physical_Object ;
    owl:subPropertyOf :occurred_in_the_presence_of ;
    diga:crm_equivalent crm:P25_moved ;
    .

:took_place_at a owl:ObjectProperty ;
    rdfs:label "took place at" ;
    skos:definition """Identifies the :Place where an :Event took place.""" ;
    schema:domainIncludes :Event ;
    schema:rangeIncludes :Place ;
    # owl:subPropertyOf :occurred_in_the_presence_of ; # this would cause a hierarchical error
    diga:crm_equivalent crm:P7_took_place_at ;
    .

:moved_to a owl:ObjectProperty ;
    rdfs:label "moved to" ;
    skos:definition """Identifies the :Place where an object is moved to.""" ;
    schema:domainIncludes :Event ;
    schema:rangeIncludes :Place ;
    owl:subPropertyOf :took_place_at ;
    diga:crm_equivalent crm:P26_moved_to ;
    .

:moved_from a owl:ObjectProperty ;
    rdfs:label "moved from" ;
    skos:definition """Identifies the :Place where an object is moved from.""" ;
    schema:domainIncludes :Event ;
    schema:rangeIncludes :Place ;
    owl:subPropertyOf :took_place_at ;
    diga:crm_equivalent crm:P27_moved_from ;
    .

:has_modified a owl:ObjectProperty ;
    rdfs:label "has modified" ;
    skos:definition """Identifies a :Man_Made_Thing modified in an :Event.""" ;
    skos:note """If a modification is applied to a non-man-made object, it is regarded as :Man_Made_Thing from that time onwards.""" ;
    schema:domainIncludes :Event ;
    schema:rangeIncludes :Physical_Man_Made_Thing ;
    owl:subPropertyOf :occurred_in_the_presence_of ;
    diga:crm_equivalent crm:P31_has_modified ;
    .

:measured a owl:ObjectProperty ;
    rdfs:label "measured" ;
    skos:definition """Specifies the item that was measured in a :Measurement event. Material and immaterial things and processes may be measured.""" ;
    schema:domainIncludes :Measurement ;
    schema:rangeIncludes :Persistent_Item ;
    owl:subPropertyOf :occurred_in_the_presence_of ;
    diga:crm_equivalent crm:P39_measured ;
    .

# Commented out. Looks like Observerations and Measurements are used differently. Observations record the property
# being measured in :observed_property_type. Measurements produce :Dimensions, and can produce multiple dimensions,
# each one for a different property. So for Observation -> :obserrved_property_type is 1-to-1, 
# vs :Measurement -> :Dimension is 1-to-many.
#
# :observed_property_type a owl:ObjectProperty ;
#     rdfs:label "observed property type" ;
#     skos:definition """Associates an instance of S4 Observation with the instance of S9 Property Type
# for which the observation provides a value or evidence, such as “concentration of nitrate”
# observed in the water from a particular borehole. """ ;
#     schema:domainIncludes :Measurement ;
#     schema:rangeIncludes :Property_Type ;
#     diga:crm_equivalent crm:O9_observed_property_type ;
#     .

:observed_dimension a owl:ObjectProperty ;
    rdfs:label "observed dimension" ;
    skos:definition """Records the :Dimension that was observed in Measurement :Event. The item measured is recorded using the :measured property of the :Event. One measurement activity may determine more than one dimension of one object.""" ;
    schema:domainIncludes :Measurement ;
    schema:rangeIncludes :Dimension ;
    diga:crm_equivalent crm:P40_observed_dimension ;
    .

:had_victim a owl:ObjectProperty ;
    rdfs:label "had victim" ;
    skos:definition """An :Actor negatively affected by an event, e.g., a person who was killed, and organization that was robbed.""" ;
    skos:note """Doesn't have a CRM equivalent.""" ;
    schema:domainIncludes :Event ;
    schema:rangeIncludes :Actor ;
    owl:subPropertyOf :had_participant ;
    .

:had_beneficiary a owl:ObjectProperty ;
    rdfs:label "had beneficiary" ;
    skos:definition """An :Actor that benefits in some way when an event occurs.""" ;
    skos:note """Doesn't have a CRM equivalent.""" ;
    schema:domainIncludes :Event ;
    schema:rangeIncludes :Actor ;
    owl:subPropertyOf :had_participant ;
    .

:had_target a owl:ObjectProperty ;
    rdfs:label "had target" ;
    skos:definition """An :Entity that was intended to be affected by an :Event.""" ;
    skos:note """For example, an attack event may have a clinic as a target, and the clinic may not have been affected in any way, e.g., it didn't get damaged or destroyed. Conversely, an :Entity may have been affected, e.g., destroyed even though it was not the target (collateral damage).""" ;
    skos:note """Doesn't have a CRM equivalent.""" ;
    schema:domainIncludes :Event ;
    schema:rangeIncludes :Actor ;
    owl:subPropertyOf :had_participant ;
    .

###
### Properties of things other than events
###

:has_condition a owl:ObjectProperty ;
    rdfs:label "has condition" ;
    skos:definition """Records a :Condition_State for some :Physical_Object.""" ;
    skos:note """CRM declares the domain as E18_Physical_Thing. Not clear whether this should be required. For example, an algorithm can be state of the art, i.e., the best one for some task.""" ;
    schema:domainIncludes :Entity ;
    schema:rangeIncludes :Condition_State ;
    diga:crm_equivalent crm:P44_has_condition ;
    .

:has_dimension a owl:ObjectProperty ;
    rdfs:label "has dimension" ;
    skos:definition """Records a :Dimension of some E70 Thing.""" ;
    skos:note """CRM declares the domain as E18_Physical_Thing. Not clear whether this should be required. For example, an algorithm can be state of the art, i.e., the best one for some task.""" ;
    schema:domainIncludes :Physical_Object ;
    schema:rangeIncludes :Dimension ;
    diga:crm_equivalent crm:P43_has_dimension ;
    .


###
### Allen's temporal relationships
###

:occurs_before a owl:ObjectProperty ;
    rdfs:label "occurs before" ;
    skos:definition """This property is the same as the "before / after" relationships of Allen’s temporal logic (Allen, 1983, pp. 832-843).""" ;
    schema:domainIncludes :Event ;
    schema:rangeIncludes :Event ;
    diga:crm_equivalent crm:P120_occurs_before ;
    .

:occurs_after a owl:ObjectProperty ;
    rdfs:label "occurs after" ;
    skos:definition """This property is the same as the "before / after" relationships of Allen’s temporal logic (Allen, 1983, pp. 832-843).""" ;
    schema:domainIncludes :Event ;
    schema:rangeIncludes :Event ;
    diga:crm_equivalent crm:P120i_occurs_after ;
    .

:meets_in_time_with a owl:ObjectProperty ;
    rdfs:label "meets in time with" ;
    skos:definition """.This property is the same as the "meets / met-by" relationships of Allen’s temporal logic (Allen, 1983, pp. 832-843).""" ;
    schema:domainIncludes :Event ;
    schema:rangeIncludes :Event ;
    diga:crm_equivalent crm:P119_meets_in_time_with ;
    .

:overlaps_in_time_with a owl:ObjectProperty ;
    rdfs:label "overlaps in time with" ;
    skos:definition """This property is the same as the "overlaps / overlapped-by" relationships of Allen’s temporal logic (Allen, 1983, pp. 832-843).""" ;
    schema:domainIncludes :Event ;
    schema:rangeIncludes :Event ;
    diga:crm_equivalent crm:P118_overlaps_in_time_with ;
    .

:occurs_during a owl:ObjectProperty ;
    rdfs:label "occurs during" ;
    skos:definition """This property is the same as the "during / includes" relationships of Allen’s temporal logic (Allen, 1983, pp. 832-843).""" ;
    schema:domainIncludes :Event ;
    schema:rangeIncludes :Event ;
    diga:crm_equivalent crm:P117_occurs_during ;
    .

:includes a owl:ObjectProperty ;
    rdfs:label "includes" ;
    skos:definition """This property is the same as the "during / includes" relationships of Allen’s temporal logic (Allen, 1983, pp. 832-843).""" ;
    schema:domainIncludes :Event ;
    schema:rangeIncludes :Event ;
    diga:crm_equivalent crm:P117i_includes ;
    .

:starts a owl:ObjectProperty ;
    rdfs:label "starts" ;
    skos:definition """This property is the same as the "starts / started-by" relationships of Allen’s temporal logic (Allen, 1983, pp. 832-843).""" ;
    schema:domainIncludes :Event ;
    schema:rangeIncludes :Event ;
    diga:crm_equivalent crm:P116_starts ;
    .

:is_started_by a owl:ObjectProperty ;
    rdfs:label "is started by" ;
    skos:definition """This property is the same as the "starts / started-by" relationships of Allen’s temporal logic (Allen, 1983, pp. 832-843).""" ;
    schema:domainIncludes :Event ;
    schema:rangeIncludes :Event ;
    diga:crm_equivalent crm:P116i_is_started_by ;
    .

:finishes a owl:ObjectProperty ;
    rdfs:label "finishes" ;
    skos:definition """This property is the same as the "finishes / finished-by" relationships of Allen’s temporal logic (Allen, 1983, pp. 832-843).""" ;
    schema:domainIncludes :Event ;
    schema:rangeIncludes :Event ;
    diga:crm_equivalent crm:P115_finishes ;
    .

:is_finished_by a owl:ObjectProperty ;
    rdfs:label "is finished by" ;
    skos:definition """This property is the same as the "finishes / finished-by" relationships of Allen’s temporal logic (Allen, 1983, pp. 832-843).""" ;
    schema:domainIncludes :Event ;
    schema:rangeIncludes :Event ;
    diga:crm_equivalent crm:P115i_is_finished_by ;
    .

:is_equal_in_time_to a owl:ObjectProperty ;
    rdfs:label "is equal in time to" ;
    skos:definition """This property is the same as the "equal" relationship of Allen’s temporal logic (Allen, 1983, pp. 832-843).""" ;
    schema:domainIncludes :Event ;
    schema:rangeIncludes :Event ;
    diga:crm_equivalent crm:P114_is_equal_in_time_to ;
    .

###
### :Time_Span properties
###

:beginning_date a owl:DatatypeProperty ;
    rdfs:label "date" ;
    skos:definition """A :Time_Span can be specified using a date e.g., 2018-05-31, and the span covers the 24 hours of the day in GMT.""" ;
    schema:domainIncludes :Time_Span ;
    schema:rangeIncludes xsd:date ;
    .

:end_date a owl:DatatypeProperty ;
    rdfs:label "date" ;
    skos:definition """""" ;
    schema:domainIncludes :Time_Span ;
    schema:rangeIncludes xsd:date ;
    .

:had_at_least_duration a owl:ObjectProperty ;
    rdfs:label "had at least duration" ;
    skos:definition """Describes the minimum length of time covered by an :Time_Span.""" ;
    schema:domainIncludes :Time_Span ;
    schema:rangeIncludes :Dimension ;
    diga:crm_equivalent crm:P83_had_at_least_duration ;
    .

:had_at_most_duration a owl:ObjectProperty ;
    rdfs:label "had at most duration" ;
    skos:definition """Describes the maximum length of time covered by an :Time_Span.""" ;
    schema:domainIncludes :Time_Span ;
    schema:rangeIncludes :Dimension ;
    diga:crm_equivalent crm:P83_had_at_most_duration ;
    .

# P81 ongoing throughout: E61 Time Primitive
:ongoing_throughout_date a owl:DatatypeProperty ;
    rdfs:label "ongoing throughout" ;
    skos:definition """""" ;
    schema:domainIncludes :Time_Span ;
    schema:rangeIncludes xsd:date ;
    .

# P82 at some time within: E61 Time Primitive
:at_some_time_within_date a owl:DatatypeProperty ;
    rdfs:label "at some time within" ;
    skos:definition """""" ;
    schema:domainIncludes :Time_Span ;
    schema:rangeIncludes xsd:date ;
    .

###
### Other properties of Events or participants
###

:religion a owl:ObjectProperty ;
    rdfs:label "religion" ;
    skos:definition """Records the religion of an :Actor.""" ;
    schema:domainIncludes :Actor ;
    schema:rangeIncludes :Religion ;
    .

:nationality a owl:ObjectProperty ;
    rdfs:label "nationality" ;
    skos:definition """Records the nationality of an :Actor.""" ;
    schema:domainIncludes :Actor ;
    schema:rangeIncludes :Country ;
    .

###
### Properties that seem appropriate for anything
###




:citation a owl:DatatypeProperty ;
    rdfs:label "citation" ;
    skos:definition """A form of provenance, records a reference to a document that provides evidence for the information associated with an entity.""" ;
    schema:domainIncludes :Entity ;
    schema:rangeIncludes xsd:string ;
    .

:topic a owl:ObjectProperty ;
    rdfs:label "topic" ;
    skos:definition """Records that the object is the :topic of the subject. Applies to any two pairs of entities.""" ;
    skos:note """In CauseEx the has_topic property is defined among Events, this seems overly contraining.""" ;
    schema:domainIncludes :Entity ;
    schema:rangeIncludes :Entity ;
    .

###
### Numeric properties
### 

:has_value a owl:DatatypeProperty ;
    rdfs:label "value" ;
    skos:definition """Records a numeric value associated with an entity.""" ;
    schema:domainIncludes :Dimension ;
    schema:rangeIncludes xsd:decimal ;
    diga:crm_equivalent crm:has_value ;
    .

:value_is_at_least a owl:DatatypeProperty ;
    rdfs:label "value is at least" ;
    skos:definition """Records a lower bound on a value, when the value is not known with certainty or the value is unknown.""" ;
    schema:domainIncludes :Dimension ;
    schema:rangeIncludes xsd:decimal ;
    .

:value_is_at_most a owl:DatatypeProperty ;
    rdfs:label "value is at most" ;
    skos:definition """Records a lower bound on a value, when the value is not known with certainty or the value is unknown.""" ;
    schema:domainIncludes :Dimension ;
    schema:rangeIncludes xsd:decimal ;
    .


###
### Text properties to describe objects
###

:label a owl:DatatypeProperty ;
    rdfs:label "label" ;
    skos:definition """A short label for an entity.""" ;
    schema:domainIncludes :Entity, :Collection;
    schema:rangeIncludes xsd:string ;
    .

:title a owl:DatatypeProperty ;
    rdfs:label "title" ;
    skos:definition """A title for an entity, typically one line of text to describe it.""" ;
    schema:domainIncludes :Entity, :Collection;
    schema:rangeIncludes xsd:string ;
    .

:description a owl:DatatypeProperty ;
    rdfs:label "description" ;
    skos:definition """A long description of an entity, typically multiple lines of text.""" ;
    schema:domainIncludes :Entity, :Collection;
    schema:rangeIncludes xsd:string ;
    .

###
### Properties for codes associated with entities
###

:code a owl:DatatypeProperty ;
    rdfs:label "code" ;
    skos:definition """A short string used as a code for an entity.""" ;
    skos:note """Examples are country codes, currency codes.""" ;
    schema:domainIncludes :Entity ;
    schema:rangeIncludes xsd:string ;
    .

:iso_code a owl:DatatypeProperty ;
    rdfs:label "ISO code" ;
    skos:definition """A sanctioned ISO code for something.""" ;
    rdfs:subPropertyOf :code ;
    .

:cameo_code a owl:DatatypeProperty ;
    rdfs:label "CAMEO code" ;
    skos:definition """A code used in the CAMEO ontology.""" ;
    skos:note """See https://www.gdeltproject.org/data.html#documentation""" ;
    rdfs:subPropertyOf :code ;
    .

:iso_country_code a owl:DatatypeProperty ;
    rdfs:label "Country ISO code" ;
    skos:definition """The ISO country code.""" ;
    rdfs:subPropertyOf :iso_code ;
    schema:domainIncludes :Place ;
    .


:adm1_code a owl:DatatypeProperty ;
    rdfs:label "ADM1 code" ;
    skos:definition """The geonames ADM1 code.""" ;
    skos:note """See http://www.geonames.org/export/codes.html.""" ;
    rdfs:subPropertyOf :iso_code ;
    .

###
### Identifiers of entities
###

:identifier a owl:DatatypeProperty ;
    rdfs:label "identifier" ;
    skos:definition """A string that uniquely identifies an entity within a domain of entities.""" ;
    skos:note """Identifiers are not ncessarily globally unique in that entities of a different type may have identical identifiers to entities in another type.  For example person identifiers may not be unique across countries.""" ;
    schema:domainIncludes :Entity ;
    schema:rangeIncludes xsd:string ;
    .

###
### Properties for places
###

:city a owl:DatatypeProperty ;
    rdfs:label "city" ;
    skos:definition """The name of a city in a country, corresponds to PPL in geonames.""" ;
    schema:domainIncludes :Place ;
    schema:rangeIncludes xsd:string ;
    .

:state a owl:DatatypeProperty ;
    rdfs:label "state" ;
    skos:definition """The name of a state or province in a country, corresponds to ADM1 in geonames.""" ;
    schema:domainIncludes :Place ;
    schema:rangeIncludes xsd:string ;
    .

:country a owl:ObjectProperty ;
    rdfs:label "country" ;
    skos:definition """The name of a country.""" ;
    schema:domainIncludes :Place ;
    schema:rangeIncludes :Country ;
    .

:region a owl:DatatypeProperty ;
    rdfs:label "region" ;
    skos:definition """The name of region in the world, not assumed to be in a controlled vocabulary.""" ;
    schema:domainIncludes :Place ;
    schema:rangeIncludes xsd:string ;
    .

:latitude a owl:DatatypeProperty ;
    rdfs:label "latitude" ;
    skos:definition """The latitude coordinate of a :Place.""" ;
    schema:domainIncludes :Place ;
    schema:rangeIncludes xsd:decimal ;
    .

:longitude a owl:DatatypeProperty ;
    rdfs:label "longitude" ;
    skos:definition """The longitude coordinate of a :Place.""" ;
    schema:domainIncludes :Place ;
    schema:rangeIncludes xsd:decimal ;
    .

:has_element a owl:ObjectProperty ;
    rdfs:label "has element" ;
    skos:definition """""" ;
    schema:domainIncludes :Collection ;
    schema:rangeIncludes :Entity ;
    .

:has_member a owl:ObjectProperty ;
    rdfs:label "has member" ;
    skos:definition """""" ;
    schema:domainIncludes :Group ;
    schema:rangeIncludes :Actor ;
    .
